moved PathORAM definitions to its own file

sim/SimExtract.v
@@ -7,6 +7,7 @@ Require Import POram.Utils.Tree.
 Require Import POram.Utils.Rationals.
 Require Import POram.Utils.Distributions.
 Require Import POram.System.PathORAM.
+Require Import POram.System.PathORAMDef.
 
 Definition empty_dict {K V} : dict K V := Dict [].
 
@@ -19,7 +20,7 @@ Fixpoint empty_oram n : oram :=
   | S m => node None (empty_oram m) (empty_oram m)
   end.
 
-Definition empty_state LOP : state := {|
+Definition empty_state `{Config} : state := {|
   state_position_map := empty_position_map;
   state_stash := empty_stash;
   state_oram := empty_oram (S LOP);
@@ -39,13 +40,13 @@ Proof.
   - simpl; congruence.
 Qed.
 
-Lemma get_all_blks_tree_empty LOP :
-  get_all_blks_tree (empty_oram LOP) = [].
+Lemma get_all_blks_tree_empty n :
+  get_all_blks_tree (empty_oram n) = [].
 Proof.
-  induction LOP.
+  induction n.
   - auto.
   - simpl.
-    rewrite IHLOP; auto.
+    rewrite IHn; auto.
 Qed.
 
 Lemma empty_oram_p_b n :
@@ -56,7 +57,7 @@ Proof.
   - split; auto.
 Qed.
 
-Lemma empty_state_wf LOP : well_formed LOP (empty_state LOP).
+Lemma empty_state_wf `{C : Config} : well_formed empty_state.
 Proof.
   split.
   - constructor.
@@ -87,28 +88,28 @@ Proof.
     reflexivity.
 Qed.
 
-Fixpoint get_traces_aux (acc : list path) (LOP : nat) (ops : list (block_id * operation)) : Poram (list path) :=
+Fixpoint get_traces_aux `{Config} (acc : list path) (ops : list (block_id * operation)) : Poram (list path) :=
   match ops with
   | [] => mreturn acc
   | (id,op) :: ops' =>
-    p <- access LOP id op;;
-    get_traces_aux (fst p :: acc) LOP ops'
+    p <- access id op;;
+    get_traces_aux (fst p :: acc) ops'
   end.
 
-Definition get_traces (LOP : nat) (ops : list (block_id * operation)) (init : state) : dist (list path) :=
-  p <- get_traces_aux [] LOP ops init;;
+Definition get_traces `{Config} (ops : list (block_id * operation)) (init : state) : dist (list path) :=
+  p <- get_traces_aux [] ops init;;
   mreturn (fst p).
 
-Fixpoint get_vals_aux (acc : list nat) (LOP : nat) (ops : list (block_id * operation)) : Poram (list nat) :=
+Fixpoint get_vals_aux `{Config} (acc : list nat) (ops : list (block_id * operation)) : Poram (list nat) :=
   match ops with
   | [] => mreturn acc
   | (id,op) :: ops' =>
-    p <- access LOP id op;;
-    get_vals_aux (snd p :: acc) LOP ops'
+    p <- access id op;;
+    get_vals_aux (snd p :: acc) ops'
   end.
 
-Definition get_vals (LOP : nat) (ops : list (block_id * operation)) (init : state) : dist (list nat) :=
-  p <- get_vals_aux [] LOP ops init;;
+Definition get_vals `{Config} (ops : list (block_id * operation)) (init : state) : dist (list nat) :=
+  p <- get_vals_aux [] ops init;;
   mreturn (List.rev (fst p)).
 
 Require Import Extraction.
