theory/System/PathORAM.v
@@ -20,2008 +20,2006 @@ Require Export POram.System.PathORAMDef.
 
 Section PORAM_PROOF.
 
-Variable LOP : nat.
+  Context `{C : Config}.
+  
+  Scheme Equality for nat.
+  Fixpoint remove_aux (lst : list block) (x : block) : list block :=
+    match lst with
+    | [] => []
+    | h :: t => 
+        if andb (Nat.eqb (block_blockid h) (block_blockid x))
+             (Nat.eqb (block_payload h) (block_payload x))
+        then t 
+        else h :: (remove_aux t x)
+    end.
 
-
-Scheme Equality for nat.
-
-Fixpoint remove_aux (lst : list block) (x : block) : list block :=
-  match lst with
-  | [] => []
-  | h :: t => 
-      if andb (Nat.eqb (block_blockid h) (block_blockid x))
-           (Nat.eqb (block_payload h) (block_payload x))
-      then t 
-      else h :: (remove_aux t x)
-  end.
-
-Fixpoint remove_list_sub (sublist : list block) (lst : list block) : list block :=
+  Fixpoint remove_list_sub (sublist : list block) (lst : list block) : list block :=
     match sublist with
     | [] => lst
     | h :: t => remove_list_sub t (remove_aux lst h)
     end.
-                 
-Fixpoint lookup_ret_data (id : block_id) (lb : list block): nat :=
-  match lb with
-  | [] => 0
-  | h :: t =>
-      if Nat.eqb (block_blockid h) id then block_payload (h%nat)
-      else lookup_ret_data id t
-  end.
-
-Definition up_oram_tr (o : oram) (stop : nat) (d_n : bucket)
-  (p : path) : oram :=
-  update_tree o stop (Some d_n) p.
-             
-Definition blocks_selection (p : path) (lvl : nat) (s : state ) : state :=
-  (* unpack the state *)
-  let m := state_position_map s in (* pos_map *) 
-  let h := state_stash s in        (* stash *)
-  let o := state_oram s in         (* oram tree *)
-  let wbs := get_write_back_blocks p h 4 lvl m in (* 4 is the capability of the bucket or equivalently the number of blocks the bucket holds *)
-  let up_h := remove_list_sub wbs h in 
-  let up_o := up_oram_tr o lvl wbs p in
-  (State m up_h up_o).
-
-(* write_back is the last for-loop, searching backwards from the bottom of the tree to seek empty slots to write candidcate blocs back *)
-
-Fixpoint write_back (s : state) (p : path) (lvl : nat) : state := 
-  match lvl with
-  | O => s 
-  | S m => write_back (blocks_selection p m s) p m
-  end.
-
-Fixpoint iterate_right {X} (start : nat) (p : path) (f : path -> nat -> X -> X) (n : nat) (x : X) : X :=
-  match n with
-  | O => x
-  | S m => f p start (iterate_right (S start) p f m x)
-  end.
-
-Definition write_back_r (start : nat) (p : path) (step : nat) (s : state):=
-  iterate_right start p blocks_selection step s.
-                        
-Lemma iterate_right_split {X} n : forall (start k : nat) (f : path -> nat -> X -> X) (p : path) (x : X),
-  iterate_right start p f (n+k) x =
-  iterate_right start p f n
-  (iterate_right (n + start) p f k x).
-Proof.
-  induction n; intros.
-  - reflexivity.
-  - simpl.
-    rewrite IHn.
-    rewrite plus_n_Sm.
-    reflexivity.
-Qed.
-
-Lemma factor_lemma {X} (L k : nat) (p : path) (f : path -> nat -> X -> X) (x : X) : (k < L)%nat ->
-  iterate_right 0 p f L x =
-    iterate_right 0 p f k
-      (f p k
-         (iterate_right (S k) p f (L - 1 - k) x)
-      ).
-Proof.
-  intro.
-  assert (L = k + S ((L - 1) - k))%nat by lia.
-  rewrite H0 at 1.
-  rewrite iterate_right_split.
-  rewrite <- (plus_n_O).
-  simpl.
-  reflexivity. 
-Qed.
-
-Definition get_pre_wb_st (id : block_id) (op : operation) (m : position_map) (h : stash ) (o : oram) (p p_new: path) :=
-  let m' := update_dict id p_new m in
-  let bkts := lookup_path_oram o p in
-  let bkt_blocks := concat bkts in
-  let h' := bkt_blocks ++ h in
-  let h'' := remove_list 
-               (fun blk => (block_blockid blk) =? id) h' in  
-  let h''' :=
-    match op with
-    | Read => h'
-    | Write d => (Block id d) ::  h''
-    end in
-  let o' := clear_path o p in 
-  State m' h''' o'.
-
-Definition get_post_wb_st (s : state) (id_path : path):=
-  write_back_r O id_path (length id_path) s.
   
-Definition get_ret_data (id : block_id)(h : stash)(p : path) (o : oram):=
-  let bkts := lookup_path_oram o p in
-  let bkt_blocks := concat bkts in
-  let h' := bkt_blocks ++ h in
-  let ret_data := lookup_ret_data id h' in
-  ret_data. 
+  Fixpoint lookup_ret_data (id : block_id) (lb : list block): nat :=
+    match lb with
+    | [] => 0
+    | h :: t =>
+        if Nat.eqb (block_blockid h) id then block_payload (h%nat)
+        else lookup_ret_data id t
+    end.
 
-Definition access (id : block_id) (op : operation) :
-  Poram (path * nat) :=
-  PST <- get ;;
-  (* unpack the state *)
-  let m := state_position_map PST in
-  let h := state_stash  PST in
-  let o := state_oram PST in 
-  (* get path for the index we are querying *)
-  let len_m := LOP in
-  let p := lookup_dict (makeBoolList false len_m) id m in
-  (* flip a bunch of coins to get the new path *)      
-  p_new <- liftT (coin_flips len_m) ;;
-  (* get the updated path oram state to put and the data to return *)
-  let n_st := get_post_wb_st (get_pre_wb_st id op m h o p p_new) p in
-  let ret_data := get_ret_data id h p o in
-  (* put the updated state back *)
-  _ <- put n_st ;;
-  (* return the path l and the return value *)
-  mreturn((p, ret_data)).
+  Definition up_oram_tr (o : oram) (stop : nat) (d_n : bucket)
+    (p : path) : oram :=
+    update_tree o stop (Some d_n) p.
+  
+  Definition blocks_selection (p : path) (lvl : nat) (s : state ) : state :=
+    (* unpack the state *)
+    let m := state_position_map s in (* pos_map *) 
+    let h := state_stash s in        (* stash *)
+    let o := state_oram s in         (* oram tree *)
+    let wbs := get_write_back_blocks p h 4 lvl m in (* 4 is the capability of the bucket or equivalently the number of blocks the bucket holds *)
+    let up_h := remove_list_sub wbs h in 
+    let up_o := up_oram_tr o lvl wbs p in
+    (State m up_h up_o).
 
-(* TODO: move to Tree.v? *)
-Fixpoint get_all_blks_tree (o : oram) : list block :=
-  match o with
-  | leaf => []
-  | node obkt o_l o_r => 
-      match obkt with
-      | None => get_all_blks_tree o_l ++ get_all_blks_tree o_r
-      | Some bkt => bkt ++ (get_all_blks_tree o_l ++ get_all_blks_tree o_r)
-      end
-  end.
+  (* write_back is the last for-loop, searching backwards from the bottom of the tree to seek empty slots to write candidcate blocs back *)
 
-Record well_formed (s : state ) : Prop := 
-  {
-    no_dup_stash : NoDup (List.map block_blockid (state_stash s)); 
-    no_dup_tree : NoDup (List.map block_blockid (get_all_blks_tree (state_oram s)));
-    tree_stash_disj : disjoint_list (List.map block_blockid (get_all_blks_tree (state_oram s)))
-                        (List.map block_blockid (state_stash s)); 
-    is_pb_tr : is_p_b_tr (state_oram s) (S LOP);
-    blk_in_path_in_tree :
-    forall id, 
-    let m := state_position_map s in
-    let p := lookup_dict (makeBoolList false LOP) id m in
-    let o := state_oram s in 
+  Fixpoint write_back (s : state) (p : path) (lvl : nat) : state := 
+    match lvl with
+    | O => s 
+    | S m => write_back (blocks_selection p m s) p m
+    end.
+
+  Fixpoint iterate_right {X} (start : nat) (p : path) (f : path -> nat -> X -> X) (n : nat) (x : X) : X :=
+    match n with
+    | O => x
+    | S m => f p start (iterate_right (S start) p f m x)
+    end.
+
+  Definition write_back_r (start : nat) (p : path) (step : nat) (s : state):=
+    iterate_right start p blocks_selection step s.
+  
+  Lemma iterate_right_split {X} n : forall (start k : nat) (f : path -> nat -> X -> X) (p : path) (x : X),
+      iterate_right start p f (n+k) x =
+        iterate_right start p f n
+          (iterate_right (n + start) p f k x).
+  Proof.
+    induction n; intros.
+    - reflexivity.
+    - simpl.
+      rewrite IHn.
+      rewrite plus_n_Sm.
+      reflexivity.
+  Qed.
+
+  Lemma factor_lemma {X} (L k : nat) (p : path) (f : path -> nat -> X -> X) (x : X) :
+    (k < L)%nat ->
+    iterate_right 0 p f L x =
+      iterate_right 0 p f k
+        (f p k
+           (iterate_right (S k) p f (L - 1 - k) x)
+        ).
+  Proof.
+    intro.
+    assert (L = k + S ((L - 1) - k))%nat by lia.
+    rewrite H0 at 1.
+    rewrite iterate_right_split.
+    rewrite <- (plus_n_O).
+    simpl.
+    reflexivity. 
+  Qed.
+
+  Definition get_pre_wb_st (id : block_id) (op : operation) (m : position_map) (h : stash ) (o : oram) (p p_new: path) :=
+    let m' := update_dict id p_new m in
     let bkts := lookup_path_oram o p in
     let bkt_blocks := concat bkts in
-    In id (List.map block_blockid (get_all_blks_tree o)) ->
-    In id (List.map block_blockid bkt_blocks);
-    path_length : 
-    let m := (state_position_map s) in
-     let len_m := LOP in 
-     forall id, length(lookup_dict (makeBoolList false len_m) id m) = LOP;
-  }.
+    let h' := bkt_blocks ++ h in
+    let h'' := remove_list 
+                 (fun blk => (block_blockid blk) =? id) h' in  
+    let h''' :=
+      match op with
+      | Read => h'
+      | Write d => (Block id d) ::  h''
+      end in
+    let o' := clear_path o p in 
+    State m' h''' o'.
 
-Definition read_access (id : block_id) : Poram (path * nat) := access id Read.
+  Definition get_post_wb_st (s : state) (id_path : path):=
+    write_back_r O id_path (length id_path) s.
+  
+  Definition get_ret_data (id : block_id)(h : stash)(p : path) (o : oram):=
+    let bkts := lookup_path_oram o p in
+    let bkt_blocks := concat bkts in
+    let h' := bkt_blocks ++ h in
+    let ret_data := lookup_ret_data id h' in
+    ret_data. 
 
-Definition write_access (id : block_id) (v : nat) : Poram (path * nat) := access id (Write v).
+  Definition access (id : block_id) (op : operation) :
+    Poram (path * nat) :=
+    PST <- get ;;
+    (* unpack the state *)
+    let m := state_position_map PST in
+    let h := state_stash  PST in
+    let o := state_oram PST in 
+    (* get path for the index we are querying *)
+    let len_m := LOP in
+    let p := lookup_dict (makeBoolList false len_m) id m in
+    (* flip a bunch of coins to get the new path *)      
+    p_new <- liftT (coin_flips len_m) ;;
+    (* get the updated path oram state to put and the data to return *)
+    let n_st := get_post_wb_st (get_pre_wb_st id op m h o p p_new) p in
+    let ret_data := get_ret_data id h p o in
+    (* put the updated state back *)
+    _ <- put n_st ;;
+    (* return the path l and the return value *)
+    mreturn((p, ret_data)).
 
-Definition write_and_read_access (id : block_id) (v : nat) : Poram (path * nat) :=
-  _ <- write_access id  v;;
-  read_access id.
+  (* TODO: move to Tree.v? *)
+  Fixpoint get_all_blks_tree (o : oram) : list block :=
+    match o with
+    | leaf => []
+    | node obkt o_l o_r => 
+        match obkt with
+        | None => get_all_blks_tree o_l ++ get_all_blks_tree o_r
+        | Some bkt => bkt ++ (get_all_blks_tree o_l ++ get_all_blks_tree o_r)
+        end
+    end.
 
-Definition has_value (v : nat) : path * nat -> Prop := fun '(_, val) => v = val.
+  Record well_formed (s : state ) : Prop := 
+    {
+      no_dup_stash : NoDup (List.map block_blockid (state_stash s)); 
+      no_dup_tree : NoDup (List.map block_blockid (get_all_blks_tree (state_oram s)));
+      tree_stash_disj : disjoint_list (List.map block_blockid (get_all_blks_tree (state_oram s)))
+                          (List.map block_blockid (state_stash s)); 
+      is_pb_tr : is_p_b_tr (state_oram s) (S LOP);
+      blk_in_path_in_tree :
+      forall id, 
+        let m := state_position_map s in
+        let p := lookup_dict (makeBoolList false LOP) id m in
+        let o := state_oram s in 
+        let bkts := lookup_path_oram o p in
+        let bkt_blocks := concat bkts in
+        In id (List.map block_blockid (get_all_blks_tree o)) ->
+        In id (List.map block_blockid bkt_blocks);
+      path_length : 
+      let m := (state_position_map s) in
+      let len_m := LOP in 
+      forall id, length(lookup_dict (makeBoolList false len_m) id m) = LOP;
+    }.
 
-Definition get_payload (dist_a : dist (path * nat * state)): nat :=
-  match peek dist_a with
-  | (_,v,_) => v
-  end.
+  Definition read_access (id : block_id) : Poram (path * nat) := access id Read.
 
-Definition blk_in_stash (id : block_id) (v : nat )(st : state) : Prop :=
-  let s := state_stash st in 
-  In (Block id v) s.
+  Definition write_access (id : block_id) (v : nat) : Poram (path * nat) := access id (Write v).
 
-(* kv-rel relation should hold whenever we have a write access that has (id, v) into the ORAM.   *)
-Definition kv_rel (id : block_id) (v : nat) (st : state) : Prop :=
-  (blk_in_stash id v st) \/ (blk_in_path id v st). (* "Come back to me" -- The bone dog in Shogun Studio *)
+  Definition write_and_read_access (id : block_id) (v : nat) : Poram (path * nat) :=
+    _ <- write_access id  v;;
+    read_access id.
 
- 
-Lemma remove_aux_lemma : forall (lst : list block) (a blk: block),
-    In blk lst ->
-    In blk (remove_aux lst a) \/ a = blk.
-Proof.
-  intros.
-  induction lst; intuition.
-  simpl.
-  destruct andb eqn: eq_cond; simpl.
-  - destruct H.
-    + right.
-      rewrite andb_true_iff in eq_cond.
-      do 2 rewrite Nat.eqb_eq in eq_cond.
-      rewrite <- H. destruct a, a0; f_equal; simpl in *; firstorder.
-    + tauto.
-  - destruct H.
-    + do 2 left; auto.
-    + apply IHlst in H. tauto.
-Qed.
-      
-Lemma remove_list_sub_lemma : forall (x : block) (sub : list block) (lst : list block),
-    In x lst ->
-    In x (remove_list_sub sub lst) \/ In x sub.
-Proof.
-  intros blk s_lst.
-  induction s_lst. 
-  - simpl.  intros. left; auto.
-  - intros. simpl remove_list_sub.
-    pose proof (IHs_lst (remove_aux lst a))%list.
-    destruct (remove_aux_lemma _ a _ H).
-    + apply H0 in H1. destruct H1.
-      * left. auto.
-      * right. right; auto.
-    + right. left; auto.
-Qed.
-        
-Lemma kv_in_list_partition:
-  forall (id : block_id) (v : nat) (s : state) (del : list block),
-    blk_in_stash id v s ->
-    (In (Block id v)
-       (remove_list_sub del (state_stash s))  \/
-    (In (Block id v) del)).
-Proof.
-  intros.
-  unfold blk_in_stash in H.
-  apply remove_list_sub_lemma.
-  auto.
-Qed.  
+  Definition has_value (v : nat) : path * nat -> Prop := fun '(_, val) => v = val.
 
+  Definition get_payload (dist_a : dist (path * nat * state)): nat :=
+    match peek dist_a with
+    | (_,v,_) => v
+    end.
 
-Lemma stash_path_combined_rel_Rd : forall (id : block_id) (v : nat) (s : state) (p_new : path),
-    kv_rel id v s ->
-    blk_in_stash id v ((get_pre_wb_st id Read (state_position_map s)
-                          (state_stash s)
-                          (state_oram s)
-                          (calc_path id s) p_new)).
-Proof.
-  intros.
-  unfold get_pre_wb_st. simpl.
-  apply in_or_app.
-  destruct H.
-  - right; auto.
-  - unfold blk_in_path in H. auto.
-Qed.
+  Definition blk_in_stash (id : block_id) (v : nat )(st : state) : Prop :=
+    let s := state_stash st in 
+    In (Block id v) s.
+
+  (* kv-rel relation should hold whenever we have a write access that has (id, v) into the ORAM.   *)
+  Definition kv_rel (id : block_id) (v : nat) (st : state) : Prop :=
+    (blk_in_stash id v st) \/ (blk_in_path id v st). 
+
+  Lemma remove_aux_lemma : forall (lst : list block) (a blk: block),
+      In blk lst ->
+      In blk (remove_aux lst a) \/ a = blk.
+  Proof.
+    intros.
+    induction lst; intuition.
+    simpl.
+    destruct andb eqn: eq_cond; simpl.
+    - destruct H.
+      + right.
+        rewrite andb_true_iff in eq_cond.
+        do 2 rewrite Nat.eqb_eq in eq_cond.
+        rewrite <- H. destruct a, a0; f_equal; simpl in *; firstorder.
+      + tauto.
+    - destruct H.
+      + do 2 left; auto.
+      + apply IHlst in H. tauto.
+  Qed.
+  
+  Lemma remove_list_sub_lemma : forall (x : block) (sub : list block) (lst : list block),
+      In x lst ->
+      In x (remove_list_sub sub lst) \/ In x sub.
+  Proof.
+    intros blk s_lst.
+    induction s_lst. 
+    - simpl.  intros. left; auto.
+    - intros. simpl remove_list_sub.
+      pose proof (IHs_lst (remove_aux lst a))%list.
+      destruct (remove_aux_lemma _ a _ H).
+      + apply H0 in H1. destruct H1.
+        * left. auto.
+        * right. right; auto.
+      + right. left; auto.
+  Qed.
+  
+  Lemma kv_in_list_partition:
+    forall (id : block_id) (v : nat) (s : state) (del : list block),
+      blk_in_stash id v s ->
+      (In (Block id v)
+         (remove_list_sub del (state_stash s))  \/
+         (In (Block id v) del)).
+  Proof.
+    intros.
+    unfold blk_in_stash in H.
+    apply remove_list_sub_lemma.
+    auto.
+  Qed.  
 
 
-Lemma stash_path_combined_rel_Wr : forall (id : block_id) (v : nat) (s : state) (p_new : path),
-    blk_in_stash id v ((get_pre_wb_st id (Write v) (state_position_map s)
-                          (state_stash s)
-                          (state_oram s)
-                          (calc_path id s) p_new)).
-Proof.
-  intros.
-  unfold get_pre_wb_st;
-  unfold blk_in_stash; simpl.
-  left; auto.
-Qed.
+  Lemma stash_path_combined_rel_Rd : forall (id : block_id) (v : nat) (s : state) (p_new : path),
+      kv_rel id v s ->
+      blk_in_stash id v ((get_pre_wb_st id Read (state_position_map s)
+                            (state_stash s)
+                            (state_oram s)
+                            (calc_path id s) p_new)).
+  Proof.
+    intros.
+    unfold get_pre_wb_st. simpl.
+    apply in_or_app.
+    destruct H.
+    - right; auto.
+    - unfold blk_in_path in H. auto.
+  Qed.
 
-Definition locate_node_in_tr (o : oram) (lvl : nat) (p : path) : option bucket :=
-  match lookup_tree o lvl p with
-  | None => None
-  | Some o => o
-  end.
 
-Definition at_lvl_in_path (o : oram ) (lvl : nat) (p : path) (x : block) : Prop :=
-  match locate_node_in_tr o lvl p with
-  | None => False
-  | Some v => In x v
-  end.
+  Lemma stash_path_combined_rel_Wr : forall (id : block_id) (v : nat) (s : state) (p_new : path),
+      blk_in_stash id v ((get_pre_wb_st id (Write v) (state_position_map s)
+                            (state_stash s)
+                            (state_oram s)
+                            (calc_path id s) p_new)).
+  Proof.
+    intros.
+    unfold get_pre_wb_st;
+      unfold blk_in_stash; simpl.
+    left; auto.
+  Qed.
 
-Lemma pos_map_stable_across_wb : forall n p s start,
-    state_position_map s = state_position_map (write_back_r start p n s).
-Proof.
-  unfold write_back_r.
-  induction n; simpl; auto.
-Qed. 
+  Definition locate_node_in_tr (o : oram) (lvl : nat) (p : path) : option bucket :=
+    match lookup_tree o lvl p with
+    | None => None
+    | Some o => o
+    end.
 
-Lemma calc_path_pos_map_same : forall id s s',
-    state_position_map s = state_position_map s' ->
-    calc_path id s = calc_path id s'.
-Proof.
-  intros.
-  unfold calc_path.
-  congruence.
-Qed.
+  Definition at_lvl_in_path (o : oram ) (lvl : nat) (p : path) (x : block) : Prop :=
+    match locate_node_in_tr o lvl p with
+    | None => False
+    | Some v => In x v
+    end.
 
-Lemma calc_path_write_bk_r_stable : forall start id s n p ,
-    calc_path id (write_back_r start p n s) = calc_path id s.
-Proof.
-  intros.
-  apply calc_path_pos_map_same.
-  symmetry.
-  apply pos_map_stable_across_wb.
-Qed.
+  Lemma pos_map_stable_across_wb : forall n p s start,
+      state_position_map s = state_position_map (write_back_r start p n s).
+  Proof.
+    unfold write_back_r.
+    induction n; simpl; auto.
+  Qed. 
 
-Lemma path_conversion : forall o lvl p p' b,
-    isEqvPath p p' lvl = true -> 
-    at_lvl_in_path o lvl p b -> at_lvl_in_path o lvl p' b.
-Proof.
-  induction o.
-  - intros. auto.
-  - intros.
-    destruct lvl; auto.
-    destruct p.
-    destruct p'; simpl in *; auto.
-    inversion H.
-    destruct b0. 
-    + destruct p'.  inversion H.
-      destruct b0.
-      * eapply IHo1; eauto. exact H.
-      * inversion H.
-    + destruct p'. inversion H.
-      destruct b0.
-      * inversion H.
-      * eapply IHo2; eauto. exact H.
-Qed.
+  Lemma calc_path_pos_map_same : forall id s s',
+      state_position_map s = state_position_map s' ->
+      calc_path id s = calc_path id s'.
+  Proof.
+    intros.
+    unfold calc_path.
+    congruence.
+  Qed.
 
-Lemma locate_comp_block_selection :
-  forall o p p' lvl lvl' dlt,
-    (lvl < lvl')%nat ->    
-    locate_node_in_tr (up_oram_tr o lvl dlt p') lvl' p =
-      locate_node_in_tr o lvl' p.
-Proof.
-  intros.
-  unfold locate_node_in_tr.
-  unfold up_oram_tr.
-  rewrite lookup_tree_update_tree; auto.
-Qed.
+  Lemma calc_path_write_bk_r_stable : forall start id s n p ,
+      calc_path id (write_back_r start p n s) = calc_path id s.
+  Proof.
+    intros.
+    apply calc_path_pos_map_same.
+    symmetry.
+    apply pos_map_stable_across_wb.
+  Qed.
 
-Lemma at_lvl_in_path_blocks_selection :
-  forall s p p' lvl lvl' b,
-  (lvl < lvl')%nat ->
-  at_lvl_in_path (state_oram s) lvl' p b ->
-  at_lvl_in_path (state_oram (blocks_selection p' lvl s)) lvl' p b.
-Proof.
-  intros.
-  unfold at_lvl_in_path in *.
-  unfold blocks_selection; simpl.
-  rewrite locate_comp_block_selection; auto.
-Qed.
-
-Lemma kv_in_delta_in_tree :
-  forall (o : oram) (id : block_id) (v : nat) (del : list block) (lvl: nat )(p :path),
-    In (Block id v) del ->
-    coord_in_bound o p lvl ->
-    at_lvl_in_path (up_oram_tr o lvl del p) lvl p (Block id v).
-Proof.
-  induction o; simpl in *; try contradiction. (* discharged the first case *)
-  - unfold at_lvl_in_path in *.
-    destruct lvl; simpl in *; auto.
-    + destruct p; simpl in *; auto.
-      destruct b; simpl in *.
-      * intros. apply IHo1; auto. (* yep I can tell that the IHp is not strong enough *)
-      * intros. apply IHo2; auto.
-Qed.
-
-Lemma path_eq_get_cand_bs : forall id v h p stop m,
-    In (Block id v) (get_cand_bs h p stop m) ->
-    isEqvPath p (lookup_dict (makeBoolList false LOP) id m) stop = true.
-Proof.
-  induction h; intros; simpl in *.
-  - exfalso; auto.
-  - destruct isEqvPath eqn : pEqv_cond.
-    + destruct H; simpl in *.
-      * rewrite H in pEqv_cond. auto.
-      * apply IHh. auto.
-    + apply IHh; auto.
-Qed.
-      
-Lemma stash_block_selection : forall p s id v lvl,
-    well_formed s ->
-    length p = LOP ->
-    Nat.le lvl LOP -> 
-    blk_in_stash id v s ->
-    blk_in_stash id v (blocks_selection p lvl s) \/
-      (at_lvl_in_path (state_oram
-                         (blocks_selection p lvl s)) lvl p (Block id v) /\
-         at_lvl_in_path (state_oram
-                           (blocks_selection p lvl s)) lvl (calc_path id s) (Block id v) 
-      ).
-Proof.
-  intros.
-  remember (blocks_selection p lvl s) as s'.
-  unfold blocks_selection in Heqs'.
-  unfold blk_in_stash in Heqs'.
-  unfold blk_in_stash.
-  rewrite Heqs'.
-  simpl.
-  remember (get_write_back_blocks p (state_stash s) 4 lvl (state_position_map s)) as dlt.
-  apply kv_in_list_partition with (del := dlt) in H2.  destruct H2.
-  - left; auto.
-  - right.
-    split.
-    + apply kv_in_delta_in_tree; auto.
-      apply pb_coord_in_bound with (k := LOP); auto.
-      * apply H.
-    + apply path_conversion with (p := p).
-      * rewrite Heqdlt in H2. unfold get_write_back_blocks in H2.
-        destruct (length (state_stash s)); try contradiction.
-        apply takeL_in in H2.
-        unfold calc_path.
-        apply path_eq_get_cand_bs with (v := v )(h := state_stash s); auto.
-      * apply kv_in_delta_in_tree; auto.
-        apply pb_coord_in_bound with (k := LOP); auto.
-        apply H.
-Qed.
-
-Definition subset_rel {X} (sub lst : list X) : Prop :=
-    forall x,
-    In x sub ->
-    In x lst.
-
-Lemma In_remove_aux : forall lst x a,
-    In x (remove_aux lst a) ->
-    In x lst.
-Proof.
-  induction lst; simpl; intros; auto.
-  destruct andb eqn: eq_cond; simpl.
-  - right; auto.
-  - destruct H; auto. right.
-    apply IHlst with (a := a0). auto.
-Qed.
-
-Lemma remove_aux_removed : forall lst b,
-    NoDup lst ->
-    ~ In b (remove_aux lst b).
-Proof.
-  induction lst; simpl; intros; auto.
-  destruct andb eqn: eq_cond.
-  - intro bp.
-    rewrite andb_true_iff in eq_cond.
-    destruct eq_cond.
-    repeat rewrite Nat.eqb_eq in *.
-    assert (a = b) by (destruct a,b; simpl in *; congruence).
-    subst.
-    inversion H; auto.
-  - intros [ | in_cond ]; subst.
-    + repeat rewrite Nat.eqb_refl in eq_cond; discriminate.
-    + eapply IHlst; eauto.
-      inversion H; auto.
-Qed.
-
-Lemma NoDup_remove_aux : forall lst x,
-    NoDup (List.map block_blockid lst) ->
-    NoDup (List.map block_blockid (remove_aux lst x)).
-Proof.
-  induction lst; simpl; intros; auto.
-  destruct andb eqn: eq_cond; simpl.
-  - inversion H; auto.
-  - apply NoDup_cons_iff. split.
-    + intro.
-      rewrite in_map_iff in H0.
-      destruct H0 as [b [Hb1 Hb2]].
-      apply In_remove_aux in Hb2.
+  Lemma path_conversion : forall o lvl p p' b,
+      isEqvPath p p' lvl = true -> 
+      at_lvl_in_path o lvl p b -> at_lvl_in_path o lvl p' b.
+  Proof.
+    induction o.
+    - intros. auto.
+    - intros.
+      destruct lvl; auto.
+      destruct p.
+      destruct p'; simpl in *; auto.
       inversion H.
-      apply H2.
-      rewrite <- Hb1.
-      apply in_map; auto.
-    + apply IHlst.
+      destruct b0. 
+      + destruct p'.  inversion H.
+        destruct b0.
+        * eapply IHo1; eauto. exact H.
+        * inversion H.
+      + destruct p'. inversion H.
+        destruct b0.
+        * inversion H.
+        * eapply IHo2; eauto. exact H.
+  Qed.
+
+  Lemma locate_comp_block_selection :
+    forall o p p' lvl lvl' dlt,
+      (lvl < lvl')%nat ->    
+      locate_node_in_tr (up_oram_tr o lvl dlt p') lvl' p =
+        locate_node_in_tr o lvl' p.
+  Proof.
+    intros.
+    unfold locate_node_in_tr.
+    unfold up_oram_tr.
+    rewrite lookup_tree_update_tree; auto.
+  Qed.
+
+  Lemma at_lvl_in_path_blocks_selection :
+    forall s p p' lvl lvl' b,
+      (lvl < lvl')%nat ->
+      at_lvl_in_path (state_oram s) lvl' p b ->
+      at_lvl_in_path (state_oram (blocks_selection p' lvl s)) lvl' p b.
+  Proof.
+    intros.
+    unfold at_lvl_in_path in *.
+    unfold blocks_selection; simpl.
+    rewrite locate_comp_block_selection; auto.
+  Qed.
+
+  Lemma kv_in_delta_in_tree :
+    forall (o : oram) (id : block_id) (v : nat) (del : list block) (lvl: nat )(p :path),
+      In (Block id v) del ->
+      coord_in_bound o p lvl ->
+      at_lvl_in_path (up_oram_tr o lvl del p) lvl p (Block id v).
+  Proof.
+    induction o; simpl in *; try contradiction. (* discharged the first case *)
+    - unfold at_lvl_in_path in *.
+      destruct lvl; simpl in *; auto.
+      + destruct p; simpl in *; auto.
+        destruct b; simpl in *.
+        * intros. apply IHo1; auto. (* yep I can tell that the IHp is not strong enough *)
+        * intros. apply IHo2; auto.
+  Qed.
+
+  Lemma path_eq_get_cand_bs : forall id v h p stop m,
+      In (Block id v) (get_cand_bs h p stop m) ->
+      isEqvPath p (lookup_dict (makeBoolList false LOP) id m) stop = true.
+  Proof.
+    induction h; intros; simpl in *.
+    - exfalso; auto.
+    - destruct isEqvPath eqn : pEqv_cond.
+      + destruct H; simpl in *.
+        * rewrite H in pEqv_cond. auto.
+        * apply IHh. auto.
+      + apply IHh; auto.
+  Qed.
+  
+  Lemma stash_block_selection : forall p s id v lvl,
+      well_formed s ->
+      length p = LOP ->
+      Nat.le lvl LOP -> 
+      blk_in_stash id v s ->
+      blk_in_stash id v (blocks_selection p lvl s) \/
+        (at_lvl_in_path (state_oram
+                           (blocks_selection p lvl s)) lvl p (Block id v) /\
+           at_lvl_in_path (state_oram
+                             (blocks_selection p lvl s)) lvl (calc_path id s) (Block id v) 
+        ).
+  Proof.
+    intros.
+    remember (blocks_selection p lvl s) as s'.
+    unfold blocks_selection in Heqs'.
+    unfold blk_in_stash in Heqs'.
+    unfold blk_in_stash.
+    rewrite Heqs'.
+    simpl.
+    remember (get_write_back_blocks p (state_stash s) 4 lvl (state_position_map s)) as dlt.
+    apply kv_in_list_partition with (del := dlt) in H2.  destruct H2.
+    - left; auto.
+    - right.
+      split.
+      + apply kv_in_delta_in_tree; auto.
+        apply pb_coord_in_bound with (k := LOP); auto.
+        * apply H.
+      + apply path_conversion with (p := p).
+        * rewrite Heqdlt in H2. unfold get_write_back_blocks in H2.
+          destruct (length (state_stash s)); try contradiction.
+          apply takeL_in in H2.
+          unfold calc_path.
+          apply path_eq_get_cand_bs with (v := v )(h := state_stash s); auto.
+        * apply kv_in_delta_in_tree; auto.
+          apply pb_coord_in_bound with (k := LOP); auto.
+          apply H.
+  Qed.
+
+  Definition subset_rel {X} (sub lst : list X) : Prop :=
+    forall x,
+      In x sub ->
+      In x lst.
+
+  Lemma In_remove_aux : forall lst x a,
+      In x (remove_aux lst a) ->
+      In x lst.
+  Proof.
+    induction lst; simpl; intros; auto.
+    destruct andb eqn: eq_cond; simpl.
+    - right; auto.
+    - destruct H; auto. right.
+      apply IHlst with (a := a0). auto.
+  Qed.
+
+  Lemma remove_aux_removed : forall lst b,
+      NoDup lst ->
+      ~ In b (remove_aux lst b).
+  Proof.
+    induction lst; simpl; intros; auto.
+    destruct andb eqn: eq_cond.
+    - intro bp.
+      rewrite andb_true_iff in eq_cond.
+      destruct eq_cond.
+      repeat rewrite Nat.eqb_eq in *.
+      assert (a = b) by (destruct a,b; simpl in *; congruence).
+      subst.
       inversion H; auto.
-Qed.
-      
-Lemma NoDup_remove_list_sub : forall (dlt lst : list block),
-    NoDup (List.map block_blockid lst) -> 
-    NoDup (List.map block_blockid (remove_list_sub dlt lst)).
-Proof.
-  induction dlt; simpl.
-  - intros; auto.
-  - intros.
-    apply IHdlt.
-    apply NoDup_remove_aux; auto.
-Qed.
+    - intros [ | in_cond ]; subst.
+      + repeat rewrite Nat.eqb_refl in eq_cond; discriminate.
+      + eapply IHlst; eauto.
+        inversion H; auto.
+  Qed.
 
-Lemma up_oram_tr_tree_or_delta o : forall id lvl dlt p,
-  In id (List.map block_blockid (get_all_blks_tree
-    (up_oram_tr o lvl dlt p))) ->
-  In id (List.map block_blockid (get_all_blks_tree o)) \/
-  In id (List.map block_blockid dlt).
-Proof.
-  induction o; simpl; intros; auto.
-  destruct data; simpl.
-  - destruct lvl; simpl in *.
-    + repeat rewrite map_app in *.
-      repeat rewrite in_app_iff in *.
-      tauto.
-    + destruct p; simpl in *.
-      * repeat rewrite map_app in *.
-        left. auto.
-      * destruct b0; simpl in *; try repeat rewrite map_app in *;
-          try repeat rewrite in_app_iff in *; try repeat destruct H; auto.
-        -- edestruct IHo1; eauto.
-        -- edestruct IHo2; eauto.
-  - destruct lvl; simpl in *.
-    + repeat rewrite map_app in *.
-      repeat rewrite in_app_iff in *.
-      tauto.
-    + destruct p; simpl in *.
-      * repeat rewrite map_app in *.
-        left. auto.
-      * destruct b; simpl in *; try repeat rewrite map_app in *;
-          try repeat rewrite in_app_iff in *; try repeat destruct H; auto.
-        -- edestruct IHo1; eauto.
-        -- edestruct IHo2; eauto.
-Qed.
-
-Lemma NoDup_up_oram_tree : forall o dlt lvl p,
-    NoDup (List.map block_blockid dlt) ->
-    NoDup (List.map block_blockid (get_all_blks_tree o)) -> 
-    disjoint_list (List.map block_blockid (get_all_blks_tree o))
-      (List.map block_blockid dlt) -> 
-    NoDup
-    (List.map block_blockid
-       (get_all_blks_tree (up_oram_tr o lvl dlt p))).
-Proof.
-  induction o; simpl; intros; auto.
-  destruct lvl; simpl; auto.
-  - destruct data; simpl; auto.
-    + apply NoDup_disjointness; auto.
-      * repeat rewrite map_app in *.
-        apply NoDup_app_remove_l in H0; auto.
-      * intros id [Hid1 Hid2].
-        apply (H1 id); split; auto.
-        rewrite map_app.
-        apply in_or_app; auto.
-    + apply NoDup_disjointness; auto.
-      * repeat rewrite map_app in *.
-        intros id [Hid1 Hid2].
-        apply (H1 id); split; auto.
-  - destruct p; simpl; auto.
-    destruct b; simpl; auto.
-    destruct data; simpl; auto.
-    + apply NoDup_disjointness; auto.
-      * repeat rewrite map_app in H0.
-        apply NoDup_app_remove_r in H0; auto.
-      * apply NoDup_disjointness.
-        -- apply IHo1; auto.
-           ++ repeat rewrite map_app in *.
-              apply NoDup_app_remove_l in H0; auto.
-              apply NoDup_app_remove_r in H0; auto.
-           ++ intros id [Hid1 Hid2].
-              apply (H1 id); split; auto.
-              repeat rewrite map_app.
-              apply in_or_app; right.
-              apply in_or_app; auto.
-        -- repeat rewrite map_app in H0.
-           do 2 apply NoDup_app_remove_l in H0; auto.
-        -- intros id [Hid1 Hid2].
-           apply up_oram_tr_tree_or_delta in Hid1.
-           destruct Hid1 as [Hid1|Hid1].
-           ++ repeat rewrite map_app in H0.
-              apply NoDup_app_remove_l in H0.
-              apply NoDup_app_disj in H0.
-              apply (H0 id); split; auto.
-           ++ apply (H1 id); split; auto.
-              repeat rewrite map_app.
-              apply in_or_app.
-              right.
-              apply in_or_app. auto.
-      * intros id [Hid1 Hid2].
-        repeat rewrite map_app in *.
-        apply in_app_or in Hid2; destruct Hid2 as [Hid2|Hid2].
-        -- apply up_oram_tr_tree_or_delta in Hid2; destruct Hid2 as [Hid2|Hid2].
-           ++ apply NoDup_app_disj in H0.
-              apply (H0 id); split; auto.
-              apply in_or_app; auto.
-           ++ apply (H1 id); split; auto.
-              apply in_or_app; left; auto.
-        -- apply NoDup_app_disj in H0.
-           apply (H0 id); split; auto.
-           apply in_or_app; right; auto.
-    + apply NoDup_disjointness.
-      * apply IHo1; auto.
-        -- rewrite map_app in H0.
-           apply NoDup_app_remove_r in H0; auto.
-        -- intros id [Hid1 Hid2].
-           apply (H1 id); split; auto.
-           rewrite map_app.
-           apply in_or_app; left; auto.
-      * rewrite map_app in H0.
-        apply NoDup_app_remove_l in H0; auto.
-      * intros id [Hid1 Hid2].
-        apply up_oram_tr_tree_or_delta in Hid1; destruct Hid1 as [Hid1|Hid1].
-        -- rewrite map_app in H0.
-           apply NoDup_app_disj in H0.
-           apply (H0 id); split; auto.
-        -- apply (H1 id); split; auto.
-           rewrite map_app.
-           apply in_or_app; right; auto.
-    + destruct data.
-      * repeat rewrite map_app in H0, H1.
-        apply NoDup_disjointness.
-        -- apply NoDup_app_remove_r in H0; auto.
-        -- apply NoDup_app_remove_l in H0.
-           apply NoDup_disjointness.
-           ++ apply NoDup_app_remove_r in H0; auto.
-           ++ apply IHo2; auto.
-              ** apply NoDup_app_remove_l in H0; auto.
-              ** intros id [Hid1 Hid2].
-                 apply (H1 id); split; auto.
-                 apply in_or_app; right.
-                 apply in_or_app; right; auto.
-           ++ intros id [Hid1 Hid2].
-              apply up_oram_tr_tree_or_delta in Hid2; destruct Hid2 as [Hid2|Hid2].
-              ** apply NoDup_app_disj in H0.
-                 apply (H0 id); split; auto.
-              ** apply (H1 id); split; auto.
-                 apply in_or_app; right.
-                 apply in_or_app; left; auto.
-        -- intros id [Hid1 Hid2].
-           apply NoDup_app_disj in H0.
-           rewrite map_app in Hid2.
-           apply in_app_or in Hid2; destruct Hid2 as [Hid2|Hid2].
-           ++ apply (H0 id); split; auto.
-              apply in_or_app; left; auto.
-           ++ apply up_oram_tr_tree_or_delta in Hid2; destruct Hid2 as [Hid2|Hid2].
-              ** apply (H0 id); split; auto.
-                 apply in_or_app; right; auto.
-              ** apply (H1 id); split; auto.
-                 apply in_or_app; left; auto.           
-      * repeat rewrite map_app in H0, H1.
-        apply NoDup_disjointness.
-        -- apply NoDup_app_remove_r in H0; auto.
-        -- apply IHo2; auto.
-           ++ apply NoDup_app_remove_l in H0; auto.
-           ++ intros id [Hid1 Hid2].
-              apply (H1 id); split; auto.
-              apply in_or_app; right; auto.
-        -- intros id [Hid1 Hid2].
-           apply up_oram_tr_tree_or_delta in Hid2; destruct Hid2 as [Hid2|Hid2].
-           ++ apply NoDup_app_disj in H0.
-              apply (H0 id); split; auto.
-           ++ apply (H1 id); split; auto.
-              apply in_or_app; left; auto.
-Qed.
-    
-Lemma map_takeL {A B} (f : A -> B) : forall n l,
-    List.map f (takeL n l) = takeL n (List.map f l).
-Proof.
-  induction n; auto.
-  intro.
-  destruct l; simpl; try reflexivity.
-  rewrite IHn. reflexivity.
-Qed.
-
-Lemma subset_rel_get_cand_bs : forall lst p lvl pos_map,
-    subset_rel (get_cand_bs lst p lvl pos_map) lst.
-Proof.
-  unfold subset_rel.
-  intros.
-  induction lst; simpl in *; auto.
-  destruct isEqvPath eqn:p_cond.
-  - inversion H.
-    + left; auto.
-    + right; apply IHlst; auto.
-  - right. apply IHlst; auto.
-Qed.
-
-Lemma NoDup_get_write_back_blocks : forall lst p lvl pos_map, 
-  NoDup (List.map block_blockid lst) ->
-  NoDup (List.map block_blockid 
-    (get_write_back_blocks p lst 4 lvl pos_map)).
-Proof.
-  unfold get_write_back_blocks. intros.
-  destruct (length lst); try constructor.
-  rewrite map_takeL.
-  apply NoDup_takeL.
-  induction lst; simpl.
-  - apply NoDup_nil.
-  - destruct isEqvPath eqn : p_cond.
-    + simpl; apply NoDup_cons_iff; split.
-      * intro pf. 
-        rewrite in_map_iff in pf.
-        destruct pf as [b [Hb1 Hb2]].
-        apply subset_rel_get_cand_bs in Hb2.
+  Lemma NoDup_remove_aux : forall lst x,
+      NoDup (List.map block_blockid lst) ->
+      NoDup (List.map block_blockid (remove_aux lst x)).
+  Proof.
+    induction lst; simpl; intros; auto.
+    destruct andb eqn: eq_cond; simpl.
+    - inversion H; auto.
+    - apply NoDup_cons_iff. split.
+      + intro.
+        rewrite in_map_iff in H0.
+        destruct H0 as [b [Hb1 Hb2]].
+        apply In_remove_aux in Hb2.
         inversion H.
         apply H2.
         rewrite <- Hb1.
-        apply in_map; auto.        
-      * apply IHlst. inversion H; auto.
-    + apply IHlst; inversion H; auto.
-Qed.
+        apply in_map; auto.
+      + apply IHlst.
+        inversion H; auto.
+  Qed.
+  
+  Lemma NoDup_remove_list_sub : forall (dlt lst : list block),
+      NoDup (List.map block_blockid lst) -> 
+      NoDup (List.map block_blockid (remove_list_sub dlt lst)).
+  Proof.
+    induction dlt; simpl.
+    - intros; auto.
+    - intros.
+      apply IHdlt.
+      apply NoDup_remove_aux; auto.
+  Qed.
 
-Lemma up_oram_tr_preserves_pb : forall o lvl dlt p n,
-    is_p_b_tr o n ->
-    is_p_b_tr (up_oram_tr o lvl dlt p) n.
-Proof.
-  intros; apply update_tree_preserves_pb; auto.
-Qed.
+  Lemma up_oram_tr_tree_or_delta o : forall id lvl dlt p,
+      In id (List.map block_blockid (get_all_blks_tree
+                                       (up_oram_tr o lvl dlt p))) ->
+      In id (List.map block_blockid (get_all_blks_tree o)) \/
+        In id (List.map block_blockid dlt).
+  Proof.
+    induction o; simpl; intros; auto.
+    destruct data; simpl.
+    - destruct lvl; simpl in *.
+      + repeat rewrite map_app in *.
+        repeat rewrite in_app_iff in *.
+        tauto.
+      + destruct p; simpl in *.
+        * repeat rewrite map_app in *.
+          left. auto.
+        * destruct b0; simpl in *; try repeat rewrite map_app in *;
+            try repeat rewrite in_app_iff in *; try repeat destruct H; auto.
+          -- edestruct IHo1; eauto.
+          -- edestruct IHo2; eauto.
+    - destruct lvl; simpl in *.
+      + repeat rewrite map_app in *.
+        repeat rewrite in_app_iff in *.
+        tauto.
+      + destruct p; simpl in *.
+        * repeat rewrite map_app in *.
+          left. auto.
+        * destruct b; simpl in *; try repeat rewrite map_app in *;
+            try repeat rewrite in_app_iff in *; try repeat destruct H; auto.
+          -- edestruct IHo1; eauto.
+          -- edestruct IHo2; eauto.
+  Qed.
 
-Lemma disjoint_weaken2 : forall dlt l lst, 
-    disjoint_list
-      (List.map block_blockid l)
-      (List.map block_blockid lst) ->
-    subset_rel dlt lst -> 
-    disjoint_list
-      (List.map block_blockid l)
-      (List.map block_blockid dlt).
-Proof.
-  intros.
-  intros id [Hid1 Hid2].
-  apply (H id); split; auto.
-  rewrite in_map_iff in *.
-  destruct Hid2 as [b [Hb1 Hb2]].
-  exists b.
-  split; auto.
-Qed.
+  Lemma NoDup_up_oram_tree : forall o dlt lvl p,
+      NoDup (List.map block_blockid dlt) ->
+      NoDup (List.map block_blockid (get_all_blks_tree o)) -> 
+      disjoint_list (List.map block_blockid (get_all_blks_tree o))
+        (List.map block_blockid dlt) -> 
+      NoDup
+        (List.map block_blockid
+           (get_all_blks_tree (up_oram_tr o lvl dlt p))).
+  Proof.
+    induction o; simpl; intros; auto.
+    destruct lvl; simpl; auto.
+    - destruct data; simpl; auto.
+      + apply NoDup_disjointness; auto.
+        * repeat rewrite map_app in *.
+          apply NoDup_app_remove_l in H0; auto.
+        * intros id [Hid1 Hid2].
+          apply (H1 id); split; auto.
+          rewrite map_app.
+          apply in_or_app; auto.
+      + apply NoDup_disjointness; auto.
+        * repeat rewrite map_app in *.
+          intros id [Hid1 Hid2].
+          apply (H1 id); split; auto.
+    - destruct p; simpl; auto.
+      destruct b; simpl; auto.
+      destruct data; simpl; auto.
+      + apply NoDup_disjointness; auto.
+        * repeat rewrite map_app in H0.
+          apply NoDup_app_remove_r in H0; auto.
+        * apply NoDup_disjointness.
+          -- apply IHo1; auto.
+             ++ repeat rewrite map_app in *.
+                apply NoDup_app_remove_l in H0; auto.
+                apply NoDup_app_remove_r in H0; auto.
+             ++ intros id [Hid1 Hid2].
+                apply (H1 id); split; auto.
+                repeat rewrite map_app.
+                apply in_or_app; right.
+                apply in_or_app; auto.
+          -- repeat rewrite map_app in H0.
+             do 2 apply NoDup_app_remove_l in H0; auto.
+          -- intros id [Hid1 Hid2].
+             apply up_oram_tr_tree_or_delta in Hid1.
+             destruct Hid1 as [Hid1|Hid1].
+             ++ repeat rewrite map_app in H0.
+                apply NoDup_app_remove_l in H0.
+                apply NoDup_app_disj in H0.
+                apply (H0 id); split; auto.
+             ++ apply (H1 id); split; auto.
+                repeat rewrite map_app.
+                apply in_or_app.
+                right.
+                apply in_or_app. auto.
+        * intros id [Hid1 Hid2].
+          repeat rewrite map_app in *.
+          apply in_app_or in Hid2; destruct Hid2 as [Hid2|Hid2].
+          -- apply up_oram_tr_tree_or_delta in Hid2; destruct Hid2 as [Hid2|Hid2].
+             ++ apply NoDup_app_disj in H0.
+                apply (H0 id); split; auto.
+                apply in_or_app; auto.
+             ++ apply (H1 id); split; auto.
+                apply in_or_app; left; auto.
+          -- apply NoDup_app_disj in H0.
+             apply (H0 id); split; auto.
+             apply in_or_app; right; auto.
+      + apply NoDup_disjointness.
+        * apply IHo1; auto.
+          -- rewrite map_app in H0.
+             apply NoDup_app_remove_r in H0; auto.
+          -- intros id [Hid1 Hid2].
+             apply (H1 id); split; auto.
+             rewrite map_app.
+             apply in_or_app; left; auto.
+        * rewrite map_app in H0.
+          apply NoDup_app_remove_l in H0; auto.
+        * intros id [Hid1 Hid2].
+          apply up_oram_tr_tree_or_delta in Hid1; destruct Hid1 as [Hid1|Hid1].
+          -- rewrite map_app in H0.
+             apply NoDup_app_disj in H0.
+             apply (H0 id); split; auto.
+          -- apply (H1 id); split; auto.
+             rewrite map_app.
+             apply in_or_app; right; auto.
+      + destruct data.
+        * repeat rewrite map_app in H0, H1.
+          apply NoDup_disjointness.
+          -- apply NoDup_app_remove_r in H0; auto.
+          -- apply NoDup_app_remove_l in H0.
+             apply NoDup_disjointness.
+             ++ apply NoDup_app_remove_r in H0; auto.
+             ++ apply IHo2; auto.
+                ** apply NoDup_app_remove_l in H0; auto.
+                ** intros id [Hid1 Hid2].
+                   apply (H1 id); split; auto.
+                   apply in_or_app; right.
+                   apply in_or_app; right; auto.
+             ++ intros id [Hid1 Hid2].
+                apply up_oram_tr_tree_or_delta in Hid2; destruct Hid2 as [Hid2|Hid2].
+                ** apply NoDup_app_disj in H0.
+                   apply (H0 id); split; auto.
+                ** apply (H1 id); split; auto.
+                   apply in_or_app; right.
+                   apply in_or_app; left; auto.
+          -- intros id [Hid1 Hid2].
+             apply NoDup_app_disj in H0.
+             rewrite map_app in Hid2.
+             apply in_app_or in Hid2; destruct Hid2 as [Hid2|Hid2].
+             ++ apply (H0 id); split; auto.
+                apply in_or_app; left; auto.
+             ++ apply up_oram_tr_tree_or_delta in Hid2; destruct Hid2 as [Hid2|Hid2].
+                ** apply (H0 id); split; auto.
+                   apply in_or_app; right; auto.
+                ** apply (H1 id); split; auto.
+                   apply in_or_app; left; auto.           
+        * repeat rewrite map_app in H0, H1.
+          apply NoDup_disjointness.
+          -- apply NoDup_app_remove_r in H0; auto.
+          -- apply IHo2; auto.
+             ++ apply NoDup_app_remove_l in H0; auto.
+             ++ intros id [Hid1 Hid2].
+                apply (H1 id); split; auto.
+                apply in_or_app; right; auto.
+          -- intros id [Hid1 Hid2].
+             apply up_oram_tr_tree_or_delta in Hid2; destruct Hid2 as [Hid2|Hid2].
+             ++ apply NoDup_app_disj in H0.
+                apply (H0 id); split; auto.
+             ++ apply (H1 id); split; auto.
+                apply in_or_app; left; auto.
+  Qed.
+  
+  Lemma map_takeL {A B} (f : A -> B) : forall n l,
+      List.map f (takeL n l) = takeL n (List.map f l).
+  Proof.
+    induction n; auto.
+    intro.
+    destruct l; simpl; try reflexivity.
+    rewrite IHn. reflexivity.
+  Qed.
 
-Lemma remove_list_sub_weaken : forall dlt lst b,
-    In b (remove_list_sub dlt lst) -> In b lst.
-Proof.
-  induction dlt; simpl; intros; auto.
-  apply IHdlt in H.
-  apply In_remove_aux in H; auto.
-Qed.  
-    
-Lemma NoDup_remove_aux_general : forall lst b,
-    NoDup lst ->
-    NoDup (remove_aux lst b).
-Proof.
-  induction lst; simpl; intros; auto.
-  destruct andb eqn: eq_cond.
-  - inversion H; auto.
-  - constructor.
-    + intro pf.
-      apply In_remove_aux in pf.
-      inversion H; auto.
-    + apply IHlst.
-      inversion H; auto.
-Qed.
+  Lemma subset_rel_get_cand_bs : forall lst p lvl pos_map,
+      subset_rel (get_cand_bs lst p lvl pos_map) lst.
+  Proof.
+    unfold subset_rel.
+    intros.
+    induction lst; simpl in *; auto.
+    destruct isEqvPath eqn:p_cond.
+    - inversion H.
+      + left; auto.
+      + right; apply IHlst; auto.
+    - right. apply IHlst; auto.
+  Qed.
 
-Lemma remove_list_sub_removed : forall dlt lst b,
-    NoDup lst ->
-    In b (remove_list_sub dlt lst) ->
-    ~ In b dlt.
-Proof.
-  induction dlt; intros; simpl in *; auto.
-  intros [ | in_cond]; subst.
-  - apply remove_list_sub_weaken in H0.
-    apply remove_aux_removed in H0; auto.    
-  - apply IHdlt in H0; auto.
-    apply NoDup_remove_aux_general; auto.
-Qed.    
+  Lemma NoDup_get_write_back_blocks : forall lst p lvl pos_map, 
+      NoDup (List.map block_blockid lst) ->
+      NoDup (List.map block_blockid 
+               (get_write_back_blocks p lst 4 lvl pos_map)).
+  Proof.
+    unfold get_write_back_blocks. intros.
+    destruct (length lst); try constructor.
+    rewrite map_takeL.
+    apply NoDup_takeL.
+    induction lst; simpl.
+    - apply NoDup_nil.
+    - destruct isEqvPath eqn : p_cond.
+      + simpl; apply NoDup_cons_iff; split.
+        * intro pf. 
+          rewrite in_map_iff in pf.
+          destruct pf as [b [Hb1 Hb2]].
+          apply subset_rel_get_cand_bs in Hb2.
+          inversion H.
+          apply H2.
+          rewrite <- Hb1.
+          apply in_map; auto.        
+        * apply IHlst. inversion H; auto.
+      + apply IHlst; inversion H; auto.
+  Qed.
 
-Lemma disjoint_dlt : forall o lvl dlt lst p,
-    NoDup (List.map block_blockid lst) ->
-    subset_rel dlt lst ->
-    disjoint_list
-      (List.map block_blockid (get_all_blks_tree o))
-      (List.map block_blockid lst) -> 
-    disjoint_list
-      (List.map block_blockid (get_all_blks_tree (up_oram_tr o lvl dlt p)))
-      (List.map block_blockid (remove_list_sub dlt lst)).
-Proof.
-  intros.
-  intros id [Hid1 Hid2].
-  apply up_oram_tr_tree_or_delta in Hid1.
-  destruct Hid1 as [Hid1|Hid1].
-  - apply (H1 id); split; auto.
-    rewrite in_map_iff in Hid2.
+  Lemma up_oram_tr_preserves_pb : forall o lvl dlt p n,
+      is_p_b_tr o n ->
+      is_p_b_tr (up_oram_tr o lvl dlt p) n.
+  Proof.
+    intros; apply update_tree_preserves_pb; auto.
+  Qed.
+
+  Lemma disjoint_weaken2 : forall dlt l lst, 
+      disjoint_list
+        (List.map block_blockid l)
+        (List.map block_blockid lst) ->
+      subset_rel dlt lst -> 
+      disjoint_list
+        (List.map block_blockid l)
+        (List.map block_blockid dlt).
+  Proof.
+    intros.
+    intros id [Hid1 Hid2].
+    apply (H id); split; auto.
+    rewrite in_map_iff in *.
     destruct Hid2 as [b [Hb1 Hb2]].
-    apply remove_list_sub_weaken in Hb2.
-    rewrite <- Hb1.
-    apply in_map; auto.
-  - rewrite in_map_iff in Hid1.
-    destruct Hid1 as [b [Hb1 Hb2]].
-    unfold subset_rel in H0.
-    rewrite in_map_iff in Hid2.
-    destruct Hid2 as [c [Hc1 Hc2]].
-    assert (b = c).
-    { apply H0 in Hb2.
-      apply remove_list_sub_weaken in Hc2.
-      apply NoDup_map_inj in H.
-      unfold inj_on_list in H.
-      apply (H b c); auto.
-      rewrite Hc1; auto.
-    }
-    subst.
-    apply remove_list_sub_removed in Hc2; auto.
-    eapply NoDup_map_inv; eauto.
-Qed.
+    exists b.
+    split; auto.
+  Qed.
+
+  Lemma remove_list_sub_weaken : forall dlt lst b,
+      In b (remove_list_sub dlt lst) -> In b lst.
+  Proof.
+    induction dlt; simpl; intros; auto.
+    apply IHdlt in H.
+    apply In_remove_aux in H; auto.
+  Qed.  
   
-Lemma get_write_back_blocks_subset : forall lst p lvl pos_map,
-    subset_rel (get_write_back_blocks p lst 4 lvl pos_map) lst.
-Proof.
-  unfold subset_rel.
-  intros.
-  unfold get_write_back_blocks in H.
-  destruct (length lst); try contradiction.
-  apply takeL_in in H.
-  apply subset_rel_get_cand_bs in H.
-  auto.
-Qed.
+  Lemma NoDup_remove_aux_general : forall lst b,
+      NoDup lst ->
+      NoDup (remove_aux lst b).
+  Proof.
+    induction lst; simpl; intros; auto.
+    destruct andb eqn: eq_cond.
+    - inversion H; auto.
+    - constructor.
+      + intro pf.
+        apply In_remove_aux in pf.
+        inversion H; auto.
+      + apply IHlst.
+        inversion H; auto.
+  Qed.
 
-Lemma In_path_in_tree : forall o p id,
-  In id (List.map block_blockid (concat (lookup_path_oram o p))) ->
-  In id (List.map block_blockid (get_all_blks_tree o)). 
-Proof.
-  induction o; simpl; intros; auto.
-  destruct p. 
-  - destruct data; simpl in *; auto.
-    + rewrite app_nil_r in H.
-      rewrite map_app.
-      apply in_or_app.
-      left; auto.
-    + contradiction.
-  - destruct b.
-    + destruct data.
-      * simpl in H.
-        rewrite map_app in H.
-        apply in_app_or in H.
-        repeat rewrite map_app.
-        apply in_or_app.
-        destruct H.
-        -- left; auto.
-        -- right. apply in_or_app.
-           left. eapply IHo1; eauto.
-      * rewrite map_app. 
-        apply in_or_app.
-        left.
-        eapply IHo1; eauto.
-    + destruct data.
-      * simpl in H.
-        rewrite map_app in H.
-        apply in_app_or in H.
-        repeat rewrite map_app.
-        apply in_or_app.
-        destruct H.
-        -- left; auto.
-        -- right. apply in_or_app.
-           right. eapply IHo2; eauto.
-      * rewrite map_app. 
-        apply in_or_app.
-        right.
-        eapply IHo2; eauto.
-Qed.
+  Lemma remove_list_sub_removed : forall dlt lst b,
+      NoDup lst ->
+      In b (remove_list_sub dlt lst) ->
+      ~ In b dlt.
+  Proof.
+    induction dlt; intros; simpl in *; auto.
+    intros [ | in_cond]; subst.
+    - apply remove_list_sub_weaken in H0.
+      apply remove_aux_removed in H0; auto.    
+    - apply IHdlt in H0; auto.
+      apply NoDup_remove_aux_general; auto.
+  Qed.    
 
-Lemma in_up_oram_tr : forall o id lvl dlt p p',
-    NoDup (List.map block_blockid (get_all_blks_tree o)) ->
-    In id (List.map block_blockid (get_all_blks_tree (up_oram_tr o lvl dlt p'))) ->
-    In id (List.map block_blockid (concat (lookup_path_oram o p))) ->
-    In id (List.map block_blockid (concat (lookup_path_oram (up_oram_tr o lvl dlt p') p))).
-Proof.
-  induction o; simpl; intros; auto.
-  destruct lvl; simpl in *.
-  - destruct p; simpl in *.
-    + rewrite app_nil_r.
-      rewrite map_app in *.
-      apply in_app_or in H0.
-      destruct H0; auto.
-      destruct data.
-      * simpl in H1.
-        rewrite app_nil_r in H1.
-        rewrite map_app in H.
-        apply NoDup_app_disj in H.
-        elim (H id); split; auto.
-      * destruct H1.
-    + destruct b; simpl; auto.
-      * destruct data; simpl; repeat rewrite map_app in *.
-        -- apply in_app_or in H0.
-           destruct H0.
-           ++ apply in_or_app.
-              left; auto.
-           ++ simpl in H1.
-              rewrite map_app in *.
-              apply in_app_or in H1.
-              apply in_or_app.
-              destruct H1.
-              ** apply NoDup_app_disj in H.
-                 elim (H id); split; auto.
-              ** right; auto.
-        -- apply in_app_or in H0.
-           destruct H0.
-           ++ apply in_or_app.
-              left; auto.
-           ++ apply in_or_app.
-              right; auto.
-      * destruct data; simpl; repeat rewrite map_app in *.
-        -- apply in_app_or in H0.
-           destruct H0.
-           ++ apply in_or_app.
-              left; auto.
-           ++ simpl in H1.
-              rewrite map_app in *.
-              apply in_app_or in H1.
-              apply in_or_app.
-              destruct H1.
-              ** apply NoDup_app_disj in H.
-                 elim (H id); split; auto.
-              ** right; auto.
-        -- apply in_app_or in H0.
-           destruct H0.
-           ++ apply in_or_app.
-              left; auto.
-           ++ apply in_or_app.
-              right; auto.
-  - destruct p; simpl; auto.
-    + destruct p'; simpl.
-      * destruct data; simpl in *; auto.
-      * destruct b; simpl in *; auto.
-    + destruct p'; simpl in *; auto.
-      destruct b; simpl in *; auto.
-      * destruct b0; simpl in *; auto.
-        destruct data; simpl in *; auto; repeat rewrite map_app in *.
-        -- apply in_or_app.
-           apply in_app_or in H1.
-           destruct H1.
-           ++ left. auto.
-           ++ right. apply IHo1; auto.
-              ** apply NoDup_app_remove_l in H.
-                 apply NoDup_app_remove_r in H; auto.
-              ** apply in_app_or in H0.
-                 destruct H0.
-                 --- apply In_path_in_tree in H1.
-                     apply NoDup_app_disj in H.
-                     elim (H id); split; auto.
-                     apply in_or_app; left; auto.
-                 --- apply in_app_or in H0.
-                     destruct H0; auto.
-                     apply NoDup_app_remove_l in H.
-                     apply NoDup_app_disj in H.
-                     elim (H id); split; auto.
-                     apply In_path_in_tree in H1; auto.
-        -- apply IHo1; auto.
-           ++ apply NoDup_app_remove_r in H; auto.
-           ++ apply in_app_or in H0.
-              destruct H0; auto.
-              apply NoDup_app_disj in H.
-              elim (H id); split; auto.
-              apply In_path_in_tree in H1; auto.
-      * destruct b0; simpl in *; auto.
-        destruct data; simpl in *; auto; repeat rewrite map_app in *.
-        -- apply in_or_app.
-           apply in_app_or in H1.
-           destruct H1.
-           ++ left. auto.
-           ++ right. apply IHo2; auto.
-              ** do 2 apply NoDup_app_remove_l in H; auto.
-              ** apply in_app_or in H0.
-                 destruct H0.
-                 --- apply In_path_in_tree in H1.
-                     apply NoDup_app_disj in H.
-                     elim (H id); split; auto.
-                     apply in_or_app; right; auto.
-                 --- apply in_app_or in H0.
-                     destruct H0; auto.
-                     apply NoDup_app_remove_l in H.
-                     apply NoDup_app_disj in H.
-                     elim (H id); split; auto.
-                     apply In_path_in_tree in H1; auto.
-        -- apply IHo2; auto.
-           ++ apply NoDup_app_remove_l in H; auto.
-           ++ apply in_app_or in H0.
-              destruct H0; auto.
-              apply NoDup_app_disj in H.
-              elim (H id); split; auto.
-              apply In_path_in_tree in H1; auto.
-Qed.
-
-Lemma get_write_back_blocks_pos_map : forall id p stsh lvl pos_map,
-  In id (List.map block_blockid
-    (get_write_back_blocks p stsh 4 lvl pos_map)) ->
-  let p' := lookup_dict (makeBoolList false LOP) id pos_map in
-  isEqvPath p p' lvl = true.
-Proof.
-  intros.
-  unfold p'.
-  rewrite in_map_iff in H.
-  destruct H as [b [Hb1 Hb2]].
-  unfold get_write_back_blocks in Hb2.
-  destruct (length stsh); auto.
-  apply takeL_in in Hb2.
-  induction stsh; simpl in *; auto.
-  destruct isEqvPath eqn:p_cond; auto.
-  destruct Hb2; auto.
-  rewrite H in p_cond.
-  rewrite Hb1 in p_cond; auto.
-Qed.
-
-Lemma isEqvPath_lookup_path_oram : forall o n id lvl dlt p p',
-    is_p_b_tr o (S n) ->
-    length p = n ->
-    length p' = n ->
-    (lvl < n)%nat ->
-    In id (List.map block_blockid dlt) ->
-    isEqvPath p p' lvl = true ->
-    In id (List.map block_blockid
-             (concat (lookup_path_oram
-                        (up_oram_tr o lvl dlt p) p'))).
-Proof.
-  induction o; simpl; intros; auto.
-  destruct lvl; simpl; auto.
-  - destruct p'; simpl; auto.
-    + rewrite app_nil_r; auto.
-    + destruct b; simpl; rewrite map_app; apply in_or_app; left; auto.
-  - destruct p; simpl; auto.
-    + simpl in H0. lia.
-    + destruct b; simpl; auto.
-      * destruct p'; simpl; auto.
-        -- simpl in H1. lia.
-        -- destruct b; [|discriminate].
-           destruct data.
-           ++ simpl.
-              rewrite map_app.
-              apply in_or_app; right.
-              destruct n as [|k]; [simpl in *; discriminate|].
-              destruct H.
-              apply IHo1 with (n := k); auto. lia.
-           ++ destruct n as [|k]; [simpl in *; discriminate|].
-              destruct H.
-              apply IHo1 with (n := k); auto. lia.
-      * destruct p'; simpl; auto.
-        -- simpl in H1. lia.
-        -- destruct b; [discriminate|].
-           destruct data.
-           ++ simpl.
-              rewrite map_app.
-              apply in_or_app; right.
-              destruct n as [|k]; [simpl in *; discriminate|].
-              destruct H.
-              apply IHo2 with (n := k); auto. lia.
-           ++ destruct n as [|k]; [simpl in *; discriminate|].
-              destruct H.
-              apply IHo2 with (n := k); auto. lia.
-Qed.
-          
-Lemma blocks_selection_wf : forall
-  (p : path) (lvl : nat) (s : state),
-  well_formed s ->
-  length p = LOP ->
-  (lvl < LOP)%nat ->
-  well_formed (blocks_selection p lvl s).
-Proof.
-  intros.
-  destruct H.
-  constructor; simpl.
-  - remember (get_write_back_blocks p (state_stash s) 4 lvl
-                (state_position_map s)) as dlt.
-    apply NoDup_remove_list_sub. auto.
-  - apply NoDup_up_oram_tree; auto.
-    + apply NoDup_get_write_back_blocks. auto.
-    + eapply disjoint_weaken2; eauto.
-      apply get_write_back_blocks_subset.
-  - apply disjoint_dlt; auto.
-    + apply get_write_back_blocks_subset.
-  - apply up_oram_tr_preserves_pb; auto.
-  - intros id Hid.
-    pose proof (Hid2 := Hid).
-    apply up_oram_tr_tree_or_delta in Hid2.
-    destruct Hid2 as [Hid2|Hid2].
-    + apply blk_in_path_in_tree0 in Hid2.
-      apply in_up_oram_tr; auto.      
-    + apply isEqvPath_lookup_path_oram with (n := LOP); auto.
-      eapply get_write_back_blocks_pos_map; eauto.
-  - auto.
-Qed.
-
-Lemma write_back_wf : forall (step start : nat) (s : state) (p : path), 
-  length p = LOP ->
-  well_formed s ->
-  Nat.le (start + step) LOP ->
-  well_formed (write_back_r start p step  s).
-Proof.
-  induction step; intros.
-  - exact H0.
-  - apply blocks_selection_wf; auto; try lia.
-    apply IHstep; auto; try lia.
-Qed.
-
-Lemma write_back_in_stash_kv_rel_aux : forall n s p id v start,
-    well_formed s ->
-    length p = LOP ->
-    Nat.le (start + n) LOP ->
-    blk_in_stash id v s ->
-    blk_in_stash id v (write_back_r start p n s) \/
-      exists k, (start <= k /\ 
-              at_lvl_in_path (state_oram (write_back_r start p n s)) k p (Block id v) /\
-              at_lvl_in_path (state_oram (write_back_r start p n s)) k (calc_path id s) (Block id v))%nat.
-Proof.
-  induction n; intros.
-  - left; auto.
-  - destruct (IHn s p id v (S start) H H0); auto; try lia.
-    + unfold write_back_r at 1.
-      simpl iterate_right at 1.
-      assert (Nat.le start LOP) by lia.
-      destruct (stash_block_selection p (write_back_r (S start) p n s) id v start) as [Hs | Hr] ; auto.
-      * apply write_back_wf; auto; try lia.
-      * right.
-        exists start; auto.
-        repeat split; auto ; try tauto.
-        destruct Hr. rewrite calc_path_write_bk_r_stable in H6.
-        exact H6.
-    + destruct H3 as [k [Hk1 Hk2]].
-      right; exists k.
-      split; [lia|].
-      unfold write_back_r; simpl iterate_right.
-      split; destruct Hk2.
-      * apply at_lvl_in_path_blocks_selection; auto.
-      * apply at_lvl_in_path_blocks_selection; auto.
-Qed. 
-
-Lemma locate_node_in_path : forall o lvl p b,
-    locate_node_in_tr o lvl p = Some b ->
-    In b (lookup_path_oram o p).
-Proof.
-  induction o.
-  - intros.
-    destruct p.
-    + inversion H.
-    + destruct b0; simpl in *; discriminate.
-  - intros.
-    destruct p.
-    + unfold locate_node_in_tr in H.
-      simpl.
-      destruct lvl; try discriminate.
-      destruct data; 
-        inversion H; subst; try discriminate. left. auto.
-    + destruct lvl; simpl in *.
-      destruct b0; simpl.
-      destruct data; simpl.
-      * left. inversion H. reflexivity.
-      * discriminate.
-      * destruct data; simpl.
-        -- left. inversion H. reflexivity.
-        -- discriminate.
-      * destruct b0; simpl in *.
-        destruct data; simpl.
-        -- right. eapply IHo1; eauto.
-        -- eapply IHo1; eauto.
-        -- destruct data; simpl.
-           ++ right.  eapply IHo2; eauto.
-           ++ eapply IHo2; eauto.
-Qed.
-
-Lemma weaken_at_lvl_in_path : forall o lvl p id v,
-  at_lvl_in_path o lvl p (Block id v) ->
-  blk_in_p id v o p.
-Proof.
-  intros.
-  unfold at_lvl_in_path in *.
-  destruct locate_node_in_tr eqn:?; [|tauto].
-  unfold blk_in_path.
-  unfold blk_in_p.
-  rewrite in_concat.
-  exists b. split; auto.
-  apply locate_node_in_path with (lvl := lvl); auto.
-Qed.
-  
-Lemma write_back_in_stash_kv_rel : forall s id v p,
-    well_formed s ->
-    length p = LOP ->
-    blk_in_stash id v s ->
-    kv_rel id v (write_back_r O p (length p) s).
-Proof.
-  intros.
-  destruct (write_back_in_stash_kv_rel_aux (length p) s p id v 0 H); auto; try lia.
-  - left; auto.
-  - destruct H2 as [k [_ Hk]].
-    right.
-    eapply weaken_at_lvl_in_path.
-    rewrite calc_path_write_bk_r_stable.
-    destruct Hk.
-    eauto.
-Qed.
-
-Lemma distribute_via_get_post_wb_st : forall (id : block_id) (v : nat) (s : state) (p : path),
-    well_formed s ->
-    length p = LOP ->
-    blk_in_stash id v s -> 
-    kv_rel id v (get_post_wb_st s p).
-Proof.
-  intros.
-  unfold get_post_wb_st.
-  apply write_back_in_stash_kv_rel; simpl; auto. 
-Qed.
-
-Lemma NoDup_path_oram : forall o p,
-    NoDup (List.map block_blockid (get_all_blks_tree o)) ->
-    NoDup (List.map block_blockid (concat (lookup_path_oram o p))).
-Proof.
-  induction o; intros.
-  - constructor.
-  - simpl in *.
-    destruct p.
-    + destruct data.
-      * simpl.
-        rewrite app_nil_r.
-        repeat rewrite map_app in H.
-        apply NoDup_app_remove_r in H; auto.
-      * constructor.
-    + destruct b.
-      * destruct data.
-        -- simpl in *.
-           apply NoDup_disjointness.
-           ++ repeat rewrite map_app in H.
-              apply NoDup_app_remove_r in H; auto.
-           ++ apply IHo1.
-              repeat rewrite map_app in H.
-              apply NoDup_app_remove_l in H; auto.
-              apply NoDup_app_remove_r in H; auto.
-           ++ intros id [Hid1 Hid2].
-              apply In_path_in_tree in Hid2.
-              repeat rewrite map_app in H.
-              rewrite app_assoc in H.
-              apply NoDup_app_remove_r in H.
-              apply (NoDup_app_disj _ _ H id); split; auto.
-        -- apply IHo1.
-           rewrite map_app in H.
-           apply NoDup_app_remove_r in H; auto.
-      * destruct data.
-        -- simpl in *.
-           apply NoDup_disjointness.
-           ++ repeat rewrite map_app in H.
-              apply NoDup_app_remove_r in H; auto.
-           ++ apply IHo2.
-              repeat rewrite map_app in H.
-              apply NoDup_app_remove_l in H; auto.
-              apply NoDup_app_remove_l in H; auto.
-           ++ intros id [Hid1 Hid2].
-              apply In_path_in_tree in Hid2.
-              repeat rewrite map_app in H.
-              apply NoDup_app_remove_mid in H.
-              apply (NoDup_app_disj _ _ H id); split; auto.
-        -- apply IHo2.
-           rewrite map_app in H.
-           apply NoDup_app_remove_l in H; auto.
-Qed. 
-
-Lemma get_all_blks_tree_clear_path_weaken : forall o id p,
-  In id (List.map block_blockid (get_all_blks_tree (clear_path o p))) ->
-  In id (List.map block_blockid (get_all_blks_tree o)).
-Proof.
-  induction o; intros.
-  - auto.
-  - destruct p; simpl in *; auto.
-    + rewrite map_app in H.
-      apply in_app_or in H.
-      destruct H.
-      * destruct data; repeat rewrite map_app.
-        -- apply in_or_app; right.
-           apply in_or_app; left; auto.
-        -- apply in_or_app; left; auto.
-      * destruct data; repeat rewrite map_app.
-        -- apply in_or_app; right.
-           apply in_or_app; right; auto.
-        -- apply in_or_app; right; auto.
-    + destruct b; simpl in *.
-      * rewrite map_app in H.
-        apply in_app_or in H.
-        destruct H.
-        -- destruct data; repeat rewrite map_app.
-           ++ apply in_or_app; right.
-              apply in_or_app; left; auto.
-              eapply IHo1; eauto.
-           ++ apply in_or_app; left.
-              eapply IHo1; eauto.
-        -- destruct data; repeat rewrite map_app.
-           ++ apply in_or_app; right.
-              apply in_or_app; right; auto.
-           ++ apply in_or_app; right; auto.
-      * destruct data; repeat rewrite map_app.
-        -- rewrite map_app in H.
-           apply in_app_or in H.
-           destruct H.
-           ++ apply in_or_app; right.
-              apply in_or_app; left; auto.
-           ++ apply in_or_app; right.
-              apply in_or_app; right.
-              eapply IHo2; eauto.
-        -- rewrite map_app in H.
-           apply in_app_or in H.
-           destruct H.
-           ++ apply in_or_app; left; auto.
-           ++ apply in_or_app; right.
-              eapply IHo2; eauto.
-Qed.
-
-Lemma NoDup_clear_path : forall o p,
-  NoDup (List.map block_blockid (get_all_blks_tree o)) ->
-  NoDup (List.map block_blockid (get_all_blks_tree (clear_path o p))).
-Proof.
-  induction o; simpl in *; intros.
-  - apply NoDup_nil.
-  - destruct p; simpl.
-    + destruct data; auto.
-      repeat rewrite map_app in *.
-      apply NoDup_app_remove_l in H. auto.
-    + destruct b; simpl.
-      * apply NoDup_disjointness.
-        -- destruct data; apply IHo1.
-           ++ repeat rewrite map_app in *.
-              apply NoDup_app_remove_l in H.
-              apply NoDup_app_remove_r in H.
-              auto.
-           ++ repeat rewrite map_app in *.
-              apply NoDup_app_remove_r in H.
-              auto.
-        -- destruct data; simpl.
-           ++ repeat rewrite map_app in *.
-              apply NoDup_app_remove_l in H.
-              apply NoDup_app_remove_l in H.
-              auto.
-           ++ repeat rewrite map_app in *.
-              apply NoDup_app_remove_l in H.
-              auto.
-        -- intros id [Hid1 Hid2].
-           apply get_all_blks_tree_clear_path_weaken in Hid1.
-           destruct data; simpl.
-           ++ repeat rewrite map_app in *.
-              apply NoDup_app_remove_l in H.
-              eapply NoDup_app_disj. exact H.
-              split; eauto.
-           ++ repeat rewrite map_app in *.
-              eapply NoDup_app_disj. exact H.
-              split; eauto.
-      * apply NoDup_disjointness.
-        -- destruct data; simpl.
-           ++ repeat rewrite map_app in *.
-              apply NoDup_app_remove_l in H.
-              apply NoDup_app_remove_r in H.
-              auto.
-           ++ repeat rewrite map_app in *.
-              apply NoDup_app_remove_r in H.
-              auto.
-        -- destruct data; apply IHo2.
-           ++ repeat rewrite map_app in *.
-              apply NoDup_app_remove_l in H.
-              apply NoDup_app_remove_l in H.
-              auto.
-           ++ repeat rewrite map_app in *.
-              apply NoDup_app_remove_l in H.
-              auto.
-        -- intros id [Hid1 Hid2].
-           apply get_all_blks_tree_clear_path_weaken in Hid2.
-           destruct data; simpl.
-           ++ repeat rewrite map_app in *.
-              apply NoDup_app_remove_l in H.
-              eapply NoDup_app_disj. exact H.
-              split; eauto.
-           ++ repeat rewrite map_app in *.
-              eapply NoDup_app_disj. exact H.
-              split; eauto.
-Qed.
-    
-Lemma clear_path_p_b_tree : forall o n p, 
-  is_p_b_tr o n -> 
-  is_p_b_tr (clear_path o p) n.
-Proof.
-  induction o; auto; intros.
-  destruct p.
-  - simpl.
-    destruct n.
-    + inversion H.
-    + split; destruct H; auto.
-  - destruct b; simpl.
-    destruct n.
-    + inversion H.
-    + inversion H. split.
-      * apply IHo1; auto.
-      * auto.
-    + destruct n; auto.
-      split.
-      * inversion H. auto.
-      * apply IHo2; auto. inversion H; auto.
-Qed.
-
-Lemma on_path_not_off_path: forall o p id,
-  NoDup (List.map block_blockid (get_all_blks_tree o)) ->
-  In id (List.map block_blockid (concat (lookup_path_oram o p))) ->
-  ~ In id (List.map block_blockid (get_all_blks_tree (clear_path o p))).
-Proof.
-  induction o; auto; intros.
-  destruct p. 
-  - destruct data; simpl in *.
-    + repeat rewrite map_app in *.
-      apply NoDup_app_disj in H.
-      intro Hid.
-      apply (H id); split.
-      * simpl in H0.
-        rewrite app_nil_r in H0; auto.
-      * auto.
-    + auto.
-  - destruct data; simpl in *.
-    + destruct b; simpl in *.
-      * repeat rewrite map_app in *. (* true *)
-        apply in_app_or in H0.
-        destruct H0.
-        -- apply NoDup_app_disj in H.
-           intro Hid.
-           apply (H id); split; auto.
-           apply in_or_app.
-           apply in_app_or in Hid.
-           destruct Hid.
-           ++ left. eapply get_all_blks_tree_clear_path_weaken. exact H1.
-           ++ right. auto.
-        -- intro.
-           apply in_app_or in H1.
-           destruct H1. 
-           ++ apply (IHo1 p id); auto.
-              apply NoDup_app_remove_l in H.
-              apply NoDup_app_remove_r in H; auto.
-           ++ apply NoDup_app_remove_l in H.
-              apply NoDup_app_disj in H.
-              apply (H id); split; auto.
-              eapply In_path_in_tree. exact H0.
-      * repeat rewrite map_app in *. (* false *)
-        apply in_app_or in H0.
-        destruct H0.
-        -- apply NoDup_app_disj in H.
-           intro Hid.
-           apply (H id); split; auto.
-           apply in_or_app.
-           apply in_app_or in Hid.
-           destruct Hid.
-           ++ left. auto.
-           ++ right. eapply get_all_blks_tree_clear_path_weaken. exact H1.
-        -- intro.
-           apply in_app_or in H1.
-           destruct H1. 
-           ++ apply (IHo2 p id); auto.
-              ** apply NoDup_app_remove_l in H.
-                 apply NoDup_app_remove_l in H; auto.
-              ** apply NoDup_app_remove_l in H.
-                 apply NoDup_app_disj in H.
-                 elim (H id); split; auto.
-                 eapply In_path_in_tree; eauto.                 
-           ++ apply (IHo2 p id); auto.
-              apply NoDup_app_remove_l in H.
-              apply NoDup_app_remove_l in H; auto.
-    + destruct b; simpl in *.
-      * repeat rewrite map_app in *.
-        pose proof (H' := H).
-        apply NoDup_app_disj in H.
-        intro Hid.
-        apply (H id); split; auto.
-        -- eapply In_path_in_tree; eauto.
-        -- apply in_app_or in Hid.
-           destruct Hid; auto.
-           elim (IHo1 p id); auto.
-           apply NoDup_app_remove_r in H'; auto.
-      * repeat rewrite map_app in *.
-        pose proof (H' := H).
-        apply NoDup_app_disj in H.
-        intro Hid.
-        apply (H id); split; auto.
-        -- apply in_app_or in Hid.
-           destruct Hid; auto.
-           elim (IHo2 p id); auto.
-           apply NoDup_app_remove_l in H'; auto.
-        -- eapply In_path_in_tree; eauto.
-Qed.
-
-Lemma disjoint_list_dlt : forall o p h,
-    disjoint_list (List.map block_blockid (get_all_blks_tree o))
-      (List.map block_blockid h) ->
-    NoDup (List.map block_blockid (get_all_blks_tree o)) -> 
-    disjoint_list (List.map block_blockid (get_all_blks_tree (clear_path o p)))
-    (List.map block_blockid (concat (lookup_path_oram o p) ++ h)).
-Proof.
-  intros.
-  intros id [Hid1 Hid2].
-  rewrite map_app in *.
-  apply in_app_or in Hid2.
-  destruct Hid2.
-  - eapply on_path_not_off_path; eauto.
-  - apply (H id); split; auto.
-    eapply get_all_blks_tree_clear_path_weaken; eauto.
-Qed.
-    
-Lemma disjoint_list_sub : forall {A} (l1 l2 l3: list A),
-  (forall x, In x l1 -> In x l2) -> 
-  disjoint_list l2 l3 ->
-  disjoint_list l1 l3.
-Proof.
-  intros.
-  unfold disjoint_list in *.
-  intros. unfold not in *.
-  firstorder.
-Qed.
-
-Lemma lookup_update_sameid : forall id m p_new, 
-    lookup_dict
-       (makeBoolList false LOP) id
-       (update_dict id p_new m) = p_new.
-Proof.
-  intros.
-  unfold lookup_dict.
-  unfold update_dict.
-  destruct m; simpl.
-  induction dict_elems as [|[k v] tl]; simpl.
-  - rewrite Nat.compare_refl; auto.
-  - destruct (id ?= k)%nat eqn:id_cond; simpl.
-    + rewrite Nat.compare_refl; auto.
-    + rewrite Nat.compare_refl; auto.
-    + rewrite id_cond.
-      exact IHtl.
-Qed.
-
-Lemma lookup_update_diffid : forall id id' m p_new,
-    id <> id' ->
-    lookup_dict
-      (makeBoolList false LOP)
-      id (update_dict id' p_new m) =
-      lookup_dict (makeBoolList false LOP) id m.
-Proof.
-  intros.
-  unfold lookup_dict.
-  unfold update_dict.
-  destruct m; simpl.
-  induction dict_elems as [|[k v] tl]; simpl.
-  - destruct (id ?= id')%nat eqn:id_cond; auto.
-    rewrite Nat.compare_eq_iff in id_cond; contradiction.
-  - destruct (id' ?= k)%nat eqn:id_cond1; simpl.
-    + rewrite Nat.compare_eq_iff in id_cond1; subst.
-      destruct (id ?= k)%nat eqn:id_cond2; auto.
-      rewrite Nat.compare_eq_iff in id_cond2; contradiction.
-    + destruct (id ?= id')%nat eqn:id_cond2; auto.
-      * rewrite Nat.compare_eq_iff in id_cond2; contradiction.
-      * rewrite <- nat_compare_lt in *.
-        assert (id < k)%nat by lia.
-        rewrite nat_compare_lt in H0.
-        rewrite H0; auto.
-    + rewrite IHtl; auto.
-Qed.
-
-Lemma lookup_off_path : forall o id p p',
-  NoDup (List.map block_blockid (get_all_blks_tree o)) ->
-  In id (List.map block_blockid (get_all_blks_tree (clear_path o p))) ->
-  In id (List.map block_blockid (concat (lookup_path_oram o p'))) ->
-  In id (List.map block_blockid (concat (lookup_path_oram (clear_path o p) p'))).
-Proof.
-  induction o; intros; simpl in *; auto.
-  destruct p; simpl in *.
-  - destruct p'.
-    + simpl.
-      destruct data; auto.
-      repeat rewrite map_app in *.
-      apply NoDup_app_disj in H.
-      simpl in H1; rewrite app_nil_r in H1.
-      apply (H id); split; auto.
-    + destruct b.
-      * destruct data; simpl in *; auto.
-        rewrite map_app in *.
-        apply in_app_or in H1.
-        destruct H1; auto.
-        apply NoDup_app_disj in H.
-        elim (H id); split; auto.
-        rewrite map_app; auto.
-      * destruct data; simpl in *; auto.
-        rewrite map_app in *.
-        apply in_app_or in H1.
-        destruct H1; auto.
-        apply NoDup_app_disj in H.
-        elim (H id); split; auto.
-        rewrite map_app; auto.
-  - destruct p'.
-    + destruct data; simpl in *.
-      * rewrite app_nil_r in H1.
-        destruct b.
-        -- simpl in *.
-           rewrite map_app in *.
-           apply NoDup_app_disj in H.
-           apply (H id); split; auto.
-           rewrite map_app.
-           rewrite in_app_iff in *.
-           destruct H0; auto.
-           left; eapply get_all_blks_tree_clear_path_weaken; eauto.
-        -- simpl in *.
-           rewrite map_app in *.
-           apply NoDup_app_disj in H.
-           apply (H id); split; auto.
-           rewrite map_app.
-           rewrite in_app_iff in *.
-           destruct H0; auto.
-           right; eapply get_all_blks_tree_clear_path_weaken; eauto.
-      * contradiction.
-    + destruct b0; simpl in *.
-      * destruct data; simpl in *.
-        -- destruct b; simpl in *.
-           ++ repeat rewrite map_app in *.
-              apply in_app_or in H1.
-              destruct H1.
-              ** apply NoDup_app_disj in H.
-                 elim (H id); split; auto.
-                 apply in_app_or in H0.
-                 apply in_or_app.
-                 destruct H0; auto.
-                 left. eapply get_all_blks_tree_clear_path_weaken; eauto.
-              ** apply IHo1; auto.
-                 --- apply NoDup_app_remove_l in H.
-                     apply NoDup_app_remove_r in H; auto.
-                 --- apply in_app_or in H0.
-                     destruct H0; auto.
-                     apply NoDup_app_remove_l in H.
-                     apply NoDup_app_disj in H.
-                     elim (H id); split; auto.
-                     eapply In_path_in_tree; eauto.
-           ++ repeat rewrite map_app in *.
-              apply in_app_or in H1.
-              destruct H1; auto.
-              apply NoDup_app_disj in H.
-              elim (H id); split; auto.
-              apply in_or_app.
-              apply in_app_or in H0.
-              destruct H0; auto.
-              right. eapply get_all_blks_tree_clear_path_weaken; eauto.
-        -- destruct b; simpl in *; auto. 
-           repeat rewrite map_app in *.
-           apply in_app_or in H0.
-           destruct H0.
-           ++ apply IHo1; auto.
-              apply NoDup_app_remove_r in H; auto.
-           ++ apply NoDup_app_disj in H.
-              elim (H id); split; auto.
-              eapply In_path_in_tree; eauto.
-      * destruct data; simpl in *.
-        -- destruct b; simpl in *.
-           ++ repeat rewrite map_app in *.
-              apply in_app_or in H1.
-              destruct H1; auto.
-              apply NoDup_app_disj in H.
-              elim (H id); split; auto.
-              apply in_or_app.
-              apply in_app_or in H0.
-              destruct H0; auto.
-              left. eapply get_all_blks_tree_clear_path_weaken; eauto.
-           ++ repeat rewrite map_app in *.
-              apply in_app_or in H1.
-              destruct H1; auto.
-              ** apply NoDup_app_disj in H.
-                 elim (H id); split; auto.
-                 apply in_or_app.
-                 apply in_app_or in H0.
-                 destruct H0; auto.
-                 right. eapply get_all_blks_tree_clear_path_weaken; eauto.
-              ** apply IHo2; auto.
-                 --- apply NoDup_app_remove_l in H.
-                     apply NoDup_app_remove_l in H; auto.
-                 --- apply in_app_or in H0.
-                     destruct H0; auto.
-                     apply NoDup_app_remove_l in H.
-                     apply NoDup_app_disj in H.
-                     elim (H id); split; auto.
-                     eapply In_path_in_tree; eauto.
-        -- destruct b; simpl in *; auto. 
-           repeat rewrite map_app in *.
-           apply in_app_or in H0.
-           destruct H0; auto.
-           ++ apply NoDup_app_disj in H.
-              elim (H id); split; auto.
-              eapply In_path_in_tree; eauto.
-           ++ apply IHo2; auto.
-              apply NoDup_app_remove_l in H; auto.
-Qed.
-
-Lemma rd_op_wf : forall (id : block_id) (m : position_map) (h : stash) (o : oram) (p p_new : path),
-    lookup_dict (makeBoolList false LOP) id m = p ->
-    well_formed (State m h o) -> length p_new = LOP -> 
-    well_formed
-      {|
-        state_position_map := update_dict id p_new m;
-        state_stash := (concat (lookup_path_oram o p) ++ h)%list;
-        state_oram := clear_path o p
-      |}.
-Proof.
-  intros.
-  destruct H0.
-  constructor; simpl in *.
-  - apply NoDup_disjointness.
-    + apply NoDup_path_oram. auto.
-    + auto.
-    + apply disjoint_list_sub with
-        (l2 := List.map block_blockid (get_all_blks_tree o)); auto.
-      intros. apply In_path_in_tree with (p := p). exact H0.
-  - apply NoDup_clear_path. auto.
-  - apply disjoint_list_dlt. auto. auto.
-  - apply clear_path_p_b_tree. auto.
-  - intros id' Hid'.
-    destruct (id =? id') eqn:id_cond.
-    + rewrite Nat.eqb_eq in id_cond. 
-      rewrite <- id_cond in *; clear id_cond.
-      pose (get_all_blks_tree_clear_path_weaken _ _ _ Hid') as Hid'2.
-      specialize (blk_in_path_in_tree0 id Hid'2).
-      rewrite H in blk_in_path_in_tree0; clear Hid'2.
-      elim on_path_not_off_path with (id := id) (o := o) (p := p); auto.
-    + rewrite Nat.eqb_neq in id_cond.
-      rewrite lookup_update_diffid; auto.
-      apply lookup_off_path; auto.
-      apply blk_in_path_in_tree0.
-      eapply get_all_blks_tree_clear_path_weaken; eauto.
-  - intro.
-    destruct (Nat.eqb id id0) eqn : id_cond.
-    + rewrite Nat.eqb_eq in id_cond. rewrite id_cond. rewrite lookup_update_sameid.
-      auto.
-    + rewrite lookup_update_diffid. auto.
-      rewrite Nat.eqb_neq in id_cond. auto.
-Qed.
-
-Lemma not_in_removed : forall l id,
- ~ In id
-  (List.map block_blockid
-     (remove_list (fun blk : block => block_blockid blk =? id)
-        l)).
-Proof.
-  intros.
-  rewrite in_map_iff.
-  intros [b [Hb1 Hb2]].
-  rewrite In_remove_list_iff in Hb2.
-  destruct Hb2 as [_ Hb2].
-  rewrite Hb1 in Hb2.
-  simpl in Hb2.
-  rewrite Nat.eqb_neq in Hb2.
-  contradiction.
-Qed.
-
-Lemma NoDup_remove_list: forall l id,
-    NoDup (List.map block_blockid l) -> 
-    NoDup
-      (List.map block_blockid
-         (remove_list (fun blk : block => block_blockid blk =? id)
-            l)).
-Proof.
-  induction l; simpl; intros; auto.
-  destruct (block_blockid a =? id).
-  - apply IHl; auto.
-    inversion H; auto.
-  - simpl.
-    constructor.
-    + intro pf.
-      rewrite in_map_iff in pf.
-      destruct pf as [b [Hb1 Hb2]].
-      rewrite In_remove_list_iff in Hb2.
-      destruct Hb2 as [Hb2 Hb3].
-      inversion H.
-      rewrite <- Hb1 in H2.
-      apply H2.
+  Lemma disjoint_dlt : forall o lvl dlt lst p,
+      NoDup (List.map block_blockid lst) ->
+      subset_rel dlt lst ->
+      disjoint_list
+        (List.map block_blockid (get_all_blks_tree o))
+        (List.map block_blockid lst) -> 
+      disjoint_list
+        (List.map block_blockid (get_all_blks_tree (up_oram_tr o lvl dlt p)))
+        (List.map block_blockid (remove_list_sub dlt lst)).
+  Proof.
+    intros.
+    intros id [Hid1 Hid2].
+    apply up_oram_tr_tree_or_delta in Hid1.
+    destruct Hid1 as [Hid1|Hid1].
+    - apply (H1 id); split; auto.
+      rewrite in_map_iff in Hid2.
+      destruct Hid2 as [b [Hb1 Hb2]].
+      apply remove_list_sub_weaken in Hb2.
+      rewrite <- Hb1.
       apply in_map; auto.
-    + apply IHl.
-      inversion H; auto.
-Qed.
-      
-Lemma wr_op_wf : forall (id : block_id) (v : nat) (m : position_map) (h : stash) (o : oram) (p p_new : path),
-    well_formed (State m h o) -> length p_new = LOP ->
-    lookup_dict (makeBoolList false LOP) id m = p ->
-    well_formed
-    {|
-      state_position_map := update_dict id p_new m;
-      state_stash :=
-        {| block_blockid := id; block_payload := v |}
-        :: remove_list (fun blk : block => block_blockid blk =? id)
-             (concat (lookup_path_oram o p) ++ h);
-      state_oram := clear_path o p
-    |}.
-Proof.
-  intros.
-  destruct H.
-  constructor; simpl in *.
-  - rewrite NoDup_cons_iff; split.
-    + apply not_in_removed.
-    + apply NoDup_remove_list.
-      apply NoDup_disjointness; auto.
-      * apply NoDup_path_oram; auto.
-      * eapply disjoint_list_sub.
-        -- apply In_path_in_tree.
-        -- auto.
-  - apply NoDup_clear_path. auto.
-  - intros id' [Hid'1 Hid'2].
-    destruct Hid'2.
-    + rewrite <- H in Hid'1; clear H.
-      apply on_path_not_off_path with (id := id) (o := o) (p := p); auto.
-      rewrite <- H1.
-      apply blk_in_path_in_tree0.
-      eapply get_all_blks_tree_clear_path_weaken; eauto.
-    + eapply disjoint_list_dlt; eauto; split; eauto.
-      rewrite in_map_iff in *.
-      destruct H as [b [Hb1 Hb2]].
-      exists b; split; auto.
-      rewrite In_remove_list_iff in Hb2; destruct Hb2; auto.
-  - apply clear_path_p_b_tree. auto.
-  - intros id' Hid'.
-    destruct (id =? id') eqn:id_cond.
-    + rewrite Nat.eqb_eq in id_cond. 
-      rewrite <- id_cond in *; clear id_cond.
-      pose (get_all_blks_tree_clear_path_weaken _ _ _ Hid') as Hid'2.
-      specialize (blk_in_path_in_tree0 id Hid'2).
-      rewrite H1 in blk_in_path_in_tree0; clear Hid'2.
-      elim on_path_not_off_path with (id := id) (o := o) (p := p); auto.
-    + rewrite Nat.eqb_neq in id_cond.
-      rewrite lookup_update_diffid; auto.
-      apply lookup_off_path; auto.
-      apply blk_in_path_in_tree0.
-      eapply get_all_blks_tree_clear_path_weaken; eauto.
-  - intro.
-    destruct (Nat.eqb id id0) eqn : id_cond.
-    + rewrite Nat.eqb_eq in id_cond. rewrite id_cond. rewrite lookup_update_sameid.
-      auto.
-    + rewrite lookup_update_diffid. auto.
-      rewrite Nat.eqb_neq in id_cond. auto.
-Qed.
-
-Lemma get_pre_wb_st_wf : forall (id : block_id) (op : operation) (m : position_map) (h : stash) (o : oram) (p p_new : path),
-    well_formed (State m h o) ->
-    length p_new = LOP ->
-    lookup_dict (makeBoolList false LOP) id m = p ->    
-    well_formed (get_pre_wb_st id op m h o p p_new).
-Proof.
-  intros.
-  unfold get_pre_wb_st.
-  destruct op. 
-  - simpl. apply rd_op_wf; auto.
-  - simpl. apply wr_op_wf; auto.
-Qed.
-
-Lemma get_post_wb_st_wf : forall (s : state) (p : path),
-    well_formed s ->
-    length p = LOP ->
-    well_formed (get_post_wb_st s p).
-Proof.
-  intros.
-  unfold get_post_wb_st.
-  apply write_back_wf; auto; lia.
-Qed.
-
-Lemma zero_sum_stsh_tr_Wr
-  (s : state) (id : block_id) (v : nat) (p p_new : path):
-  well_formed s ->
-  length p = LOP ->
-  length p_new = LOP ->
-  kv_rel id v
-    (get_post_wb_st
-       (get_pre_wb_st id (Write v)
-          (state_position_map s) (state_stash s) (state_oram s)
-          (calc_path id s) p_new) p).
-Proof.
-  intros.
-  apply distribute_via_get_post_wb_st; auto.
-  - apply get_pre_wb_st_wf; auto.
-    destruct s; auto.
-  - apply stash_path_combined_rel_Wr.
-Qed.
-        
-Lemma zero_sum_stsh_tr_Rd_rev :
-  forall (id : block_id) (v : nat) (s : state) (p p_new : path),
-    well_formed s ->
-    length p = LOP ->
-    length p_new = LOP -> 
-    kv_rel id v s  -> 
-    kv_rel id v (get_post_wb_st
-      (get_pre_wb_st id Read (state_position_map s)
-         (state_stash s)
-         (state_oram s)
-         (calc_path id s) p_new) p). 
-Proof.
-  intros.
-  apply distribute_via_get_post_wb_st; auto.
-  - apply get_pre_wb_st_wf; auto. destruct s; auto.
-  - apply stash_path_combined_rel_Rd. auto.
-Qed.
+    - rewrite in_map_iff in Hid1.
+      destruct Hid1 as [b [Hb1 Hb2]].
+      unfold subset_rel in H0.
+      rewrite in_map_iff in Hid2.
+      destruct Hid2 as [c [Hc1 Hc2]].
+      assert (b = c).
+      { apply H0 in Hb2.
+        apply remove_list_sub_weaken in Hc2.
+        apply NoDup_map_inj in H.
+        unfold inj_on_list in H.
+        apply (H b c); auto.
+        rewrite Hc1; auto.
+      }
+      subst.
+      apply remove_list_sub_removed in Hc2; auto.
+      eapply NoDup_map_inv; eauto.
+  Qed.
   
-Lemma lookup_ret_data_block_in_list (id : block_id) (v : nat) (l : list block) :
-  NoDup (List.map block_blockid l) ->
-  In (Block id v) l -> lookup_ret_data id l = v.
-Proof.
-  intro ND.
-  intros.
-  induction l; simpl; try contradiction.
-  destruct (block_blockid a =? id) eqn: id_cond.
-  - destruct H; simpl in *.
-    + rewrite H; auto.
-    + inversion ND; subst.
-      rewrite Nat.eqb_eq in id_cond.
-      rewrite id_cond in H2.
-      apply List.in_map with (f := block_blockid) in H.
-      simpl in *. contradiction.
-  - apply IHl.
-    + inversion ND; auto.
-    + destruct H; auto.
-      rewrite H in id_cond. simpl in *. rewrite Nat.eqb_neq in id_cond.
-      contradiction.
-Qed.
+  Lemma get_write_back_blocks_subset : forall lst p lvl pos_map,
+      subset_rel (get_write_back_blocks p lst 4 lvl pos_map) lst.
+  Proof.
+    unfold subset_rel.
+    intros.
+    unfold get_write_back_blocks in H.
+    destruct (length lst); try contradiction.
+    apply takeL_in in H.
+    apply subset_rel_get_cand_bs in H.
+    auto.
+  Qed.
 
-Lemma zero_sum_stsh_tr_Rd (id : block_id) (v : nat) (m : position_map) (h : stash) (o : oram) :
-  well_formed (State m h o) ->
-  kv_rel id v (State m h o) ->
-  get_ret_data id h (calc_path id (State m h o)) o = v.
-Proof.
-  simpl.
-  intros.
-  destruct H0. 
-  - (* assume in stash *)
-    apply lookup_ret_data_block_in_list.
-    + apply NoDup_disjointness; try repeat apply H.
-      * apply NoDup_path_oram. apply H.
-      * destruct H.
-        apply disjoint_list_sub with
-        (l2 := List.map block_blockid (get_all_blks_tree o)); auto.
-        intros. eapply In_path_in_tree. exact H.
-    + apply in_or_app. right. auto.
-  - (* assume in path *)
-    apply lookup_ret_data_block_in_list.
-    + apply NoDup_disjointness; try repeat apply H.
-      * apply NoDup_path_oram. apply H.
-      * destruct H.
-        apply disjoint_list_sub with
+  Lemma In_path_in_tree : forall o p id,
+      In id (List.map block_blockid (concat (lookup_path_oram o p))) ->
+      In id (List.map block_blockid (get_all_blks_tree o)). 
+  Proof.
+    induction o; simpl; intros; auto.
+    destruct p. 
+    - destruct data; simpl in *; auto.
+      + rewrite app_nil_r in H.
+        rewrite map_app.
+        apply in_or_app.
+        left; auto.
+      + contradiction.
+    - destruct b.
+      + destruct data.
+        * simpl in H.
+          rewrite map_app in H.
+          apply in_app_or in H.
+          repeat rewrite map_app.
+          apply in_or_app.
+          destruct H.
+          -- left; auto.
+          -- right. apply in_or_app.
+             left. eapply IHo1; eauto.
+        * rewrite map_app. 
+          apply in_or_app.
+          left.
+          eapply IHo1; eauto.
+      + destruct data.
+        * simpl in H.
+          rewrite map_app in H.
+          apply in_app_or in H.
+          repeat rewrite map_app.
+          apply in_or_app.
+          destruct H.
+          -- left; auto.
+          -- right. apply in_or_app.
+             right. eapply IHo2; eauto.
+        * rewrite map_app. 
+          apply in_or_app.
+          right.
+          eapply IHo2; eauto.
+  Qed.
+
+  Lemma in_up_oram_tr : forall o id lvl dlt p p',
+      NoDup (List.map block_blockid (get_all_blks_tree o)) ->
+      In id (List.map block_blockid (get_all_blks_tree (up_oram_tr o lvl dlt p'))) ->
+      In id (List.map block_blockid (concat (lookup_path_oram o p))) ->
+      In id (List.map block_blockid (concat (lookup_path_oram (up_oram_tr o lvl dlt p') p))).
+  Proof.
+    induction o; simpl; intros; auto.
+    destruct lvl; simpl in *.
+    - destruct p; simpl in *.
+      + rewrite app_nil_r.
+        rewrite map_app in *.
+        apply in_app_or in H0.
+        destruct H0; auto.
+        destruct data.
+        * simpl in H1.
+          rewrite app_nil_r in H1.
+          rewrite map_app in H.
+          apply NoDup_app_disj in H.
+          elim (H id); split; auto.
+        * destruct H1.
+      + destruct b; simpl; auto.
+        * destruct data; simpl; repeat rewrite map_app in *.
+          -- apply in_app_or in H0.
+             destruct H0.
+             ++ apply in_or_app.
+                left; auto.
+             ++ simpl in H1.
+                rewrite map_app in *.
+                apply in_app_or in H1.
+                apply in_or_app.
+                destruct H1.
+                ** apply NoDup_app_disj in H.
+                   elim (H id); split; auto.
+                ** right; auto.
+          -- apply in_app_or in H0.
+             destruct H0.
+             ++ apply in_or_app.
+                left; auto.
+             ++ apply in_or_app.
+                right; auto.
+        * destruct data; simpl; repeat rewrite map_app in *.
+          -- apply in_app_or in H0.
+             destruct H0.
+             ++ apply in_or_app.
+                left; auto.
+             ++ simpl in H1.
+                rewrite map_app in *.
+                apply in_app_or in H1.
+                apply in_or_app.
+                destruct H1.
+                ** apply NoDup_app_disj in H.
+                   elim (H id); split; auto.
+                ** right; auto.
+          -- apply in_app_or in H0.
+             destruct H0.
+             ++ apply in_or_app.
+                left; auto.
+             ++ apply in_or_app.
+                right; auto.
+    - destruct p; simpl; auto.
+      + destruct p'; simpl.
+        * destruct data; simpl in *; auto.
+        * destruct b; simpl in *; auto.
+      + destruct p'; simpl in *; auto.
+        destruct b; simpl in *; auto.
+        * destruct b0; simpl in *; auto.
+          destruct data; simpl in *; auto; repeat rewrite map_app in *.
+          -- apply in_or_app.
+             apply in_app_or in H1.
+             destruct H1.
+             ++ left. auto.
+             ++ right. apply IHo1; auto.
+                ** apply NoDup_app_remove_l in H.
+                   apply NoDup_app_remove_r in H; auto.
+                ** apply in_app_or in H0.
+                   destruct H0.
+                   --- apply In_path_in_tree in H1.
+                       apply NoDup_app_disj in H.
+                       elim (H id); split; auto.
+                       apply in_or_app; left; auto.
+                   --- apply in_app_or in H0.
+                       destruct H0; auto.
+                       apply NoDup_app_remove_l in H.
+                       apply NoDup_app_disj in H.
+                       elim (H id); split; auto.
+                       apply In_path_in_tree in H1; auto.
+          -- apply IHo1; auto.
+             ++ apply NoDup_app_remove_r in H; auto.
+             ++ apply in_app_or in H0.
+                destruct H0; auto.
+                apply NoDup_app_disj in H.
+                elim (H id); split; auto.
+                apply In_path_in_tree in H1; auto.
+        * destruct b0; simpl in *; auto.
+          destruct data; simpl in *; auto; repeat rewrite map_app in *.
+          -- apply in_or_app.
+             apply in_app_or in H1.
+             destruct H1.
+             ++ left. auto.
+             ++ right. apply IHo2; auto.
+                ** do 2 apply NoDup_app_remove_l in H; auto.
+                ** apply in_app_or in H0.
+                   destruct H0.
+                   --- apply In_path_in_tree in H1.
+                       apply NoDup_app_disj in H.
+                       elim (H id); split; auto.
+                       apply in_or_app; right; auto.
+                   --- apply in_app_or in H0.
+                       destruct H0; auto.
+                       apply NoDup_app_remove_l in H.
+                       apply NoDup_app_disj in H.
+                       elim (H id); split; auto.
+                       apply In_path_in_tree in H1; auto.
+          -- apply IHo2; auto.
+             ++ apply NoDup_app_remove_l in H; auto.
+             ++ apply in_app_or in H0.
+                destruct H0; auto.
+                apply NoDup_app_disj in H.
+                elim (H id); split; auto.
+                apply In_path_in_tree in H1; auto.
+  Qed.
+
+  Lemma get_write_back_blocks_pos_map : forall id p stsh lvl pos_map,
+      In id (List.map block_blockid
+               (get_write_back_blocks p stsh 4 lvl pos_map)) ->
+      let p' := lookup_dict (makeBoolList false LOP) id pos_map in
+      isEqvPath p p' lvl = true.
+  Proof.
+    intros.
+    unfold p'.
+    rewrite in_map_iff in H.
+    destruct H as [b [Hb1 Hb2]].
+    unfold get_write_back_blocks in Hb2.
+    destruct (length stsh); auto.
+    apply takeL_in in Hb2.
+    induction stsh; simpl in *; auto.
+    destruct isEqvPath eqn:p_cond; auto.
+    destruct Hb2; auto.
+    rewrite H in p_cond.
+    rewrite Hb1 in p_cond; auto.
+  Qed.
+
+  Lemma isEqvPath_lookup_path_oram : forall o n id lvl dlt p p',
+      is_p_b_tr o (S n) ->
+      length p = n ->
+      length p' = n ->
+      (lvl < n)%nat ->
+      In id (List.map block_blockid dlt) ->
+      isEqvPath p p' lvl = true ->
+      In id (List.map block_blockid
+               (concat (lookup_path_oram
+                          (up_oram_tr o lvl dlt p) p'))).
+  Proof.
+    induction o; simpl; intros; auto.
+    destruct lvl; simpl; auto.
+    - destruct p'; simpl; auto.
+      + rewrite app_nil_r; auto.
+      + destruct b; simpl; rewrite map_app; apply in_or_app; left; auto.
+    - destruct p; simpl; auto.
+      + simpl in H0. lia.
+      + destruct b; simpl; auto.
+        * destruct p'; simpl; auto.
+          -- simpl in H1. lia.
+          -- destruct b; [|discriminate].
+             destruct data.
+             ++ simpl.
+                rewrite map_app.
+                apply in_or_app; right.
+                destruct n as [|k]; [simpl in *; discriminate|].
+                destruct H.
+                apply IHo1 with (n := k); auto. lia.
+             ++ destruct n as [|k]; [simpl in *; discriminate|].
+                destruct H.
+                apply IHo1 with (n := k); auto. lia.
+        * destruct p'; simpl; auto.
+          -- simpl in H1. lia.
+          -- destruct b; [discriminate|].
+             destruct data.
+             ++ simpl.
+                rewrite map_app.
+                apply in_or_app; right.
+                destruct n as [|k]; [simpl in *; discriminate|].
+                destruct H.
+                apply IHo2 with (n := k); auto. lia.
+             ++ destruct n as [|k]; [simpl in *; discriminate|].
+                destruct H.
+                apply IHo2 with (n := k); auto. lia.
+  Qed.
+  
+  Lemma blocks_selection_wf : forall
+      (p : path) (lvl : nat) (s : state),
+      well_formed s ->
+      length p = LOP ->
+      (lvl < LOP)%nat ->
+      well_formed (blocks_selection p lvl s).
+  Proof.
+    intros.
+    destruct H.
+    constructor; simpl.
+    - remember (get_write_back_blocks p (state_stash s) 4 lvl
+                  (state_position_map s)) as dlt.
+      apply NoDup_remove_list_sub. auto.
+    - apply NoDup_up_oram_tree; auto.
+      + apply NoDup_get_write_back_blocks. auto.
+      + eapply disjoint_weaken2; eauto.
+        apply get_write_back_blocks_subset.
+    - apply disjoint_dlt; auto.
+      + apply get_write_back_blocks_subset.
+    - apply up_oram_tr_preserves_pb; auto.
+    - intros id Hid.
+      pose proof (Hid2 := Hid).
+      apply up_oram_tr_tree_or_delta in Hid2.
+      destruct Hid2 as [Hid2|Hid2].
+      + apply blk_in_path_in_tree0 in Hid2.
+        apply in_up_oram_tr; auto.      
+      + apply isEqvPath_lookup_path_oram with (n := LOP); auto.
+        eapply get_write_back_blocks_pos_map; eauto.
+    - auto.
+  Qed.
+
+  Lemma write_back_wf : forall (step start : nat) (s : state) (p : path), 
+      length p = LOP ->
+      well_formed s ->
+      Nat.le (start + step) LOP ->
+      well_formed (write_back_r start p step  s).
+  Proof.
+    induction step; intros.
+    - exact H0.
+    - apply blocks_selection_wf; auto; try lia.
+      apply IHstep; auto; try lia.
+  Qed.
+
+  Lemma write_back_in_stash_kv_rel_aux : forall n s p id v start,
+      well_formed s ->
+      length p = LOP ->
+      Nat.le (start + n) LOP ->
+      blk_in_stash id v s ->
+      blk_in_stash id v (write_back_r start p n s) \/
+        exists k, (start <= k /\ 
+                at_lvl_in_path (state_oram (write_back_r start p n s)) k p (Block id v) /\
+                at_lvl_in_path (state_oram (write_back_r start p n s)) k (calc_path id s) (Block id v))%nat.
+  Proof.
+    induction n; intros.
+    - left; auto.
+    - destruct (IHn s p id v (S start) H H0); auto; try lia.
+      + unfold write_back_r at 1.
+        simpl iterate_right at 1.
+        assert (Nat.le start LOP) by lia.
+        destruct (stash_block_selection p (write_back_r (S start) p n s) id v start) as [Hs | Hr] ; auto.
+        * apply write_back_wf; auto; try lia.
+        * right.
+          exists start; auto.
+          repeat split; auto ; try tauto.
+          destruct Hr. rewrite calc_path_write_bk_r_stable in H6.
+          exact H6.
+      + destruct H3 as [k [Hk1 Hk2]].
+        right; exists k.
+        split; [lia|].
+        unfold write_back_r; simpl iterate_right.
+        split; destruct Hk2.
+        * apply at_lvl_in_path_blocks_selection; auto.
+        * apply at_lvl_in_path_blocks_selection; auto.
+  Qed. 
+
+  Lemma locate_node_in_path : forall o lvl p b,
+      locate_node_in_tr o lvl p = Some b ->
+      In b (lookup_path_oram o p).
+  Proof.
+    induction o.
+    - intros.
+      destruct p.
+      + inversion H.
+      + destruct b0; simpl in *; discriminate.
+    - intros.
+      destruct p.
+      + unfold locate_node_in_tr in H.
+        simpl.
+        destruct lvl; try discriminate.
+        destruct data; 
+          inversion H; subst; try discriminate. left. auto.
+      + destruct lvl; simpl in *.
+        destruct b0; simpl.
+        destruct data; simpl.
+        * left. inversion H. reflexivity.
+        * discriminate.
+        * destruct data; simpl.
+          -- left. inversion H. reflexivity.
+          -- discriminate.
+        * destruct b0; simpl in *.
+          destruct data; simpl.
+          -- right. eapply IHo1; eauto.
+          -- eapply IHo1; eauto.
+          -- destruct data; simpl.
+             ++ right.  eapply IHo2; eauto.
+             ++ eapply IHo2; eauto.
+  Qed.
+
+  Lemma weaken_at_lvl_in_path : forall o lvl p id v,
+      at_lvl_in_path o lvl p (Block id v) ->
+      blk_in_p id v o p.
+  Proof.
+    intros.
+    unfold at_lvl_in_path in *.
+    destruct locate_node_in_tr eqn:?; [|tauto].
+    unfold blk_in_path.
+    unfold blk_in_p.
+    rewrite in_concat.
+    exists b. split; auto.
+    apply locate_node_in_path with (lvl := lvl); auto.
+  Qed.
+  
+  Lemma write_back_in_stash_kv_rel : forall s id v p,
+      well_formed s ->
+      length p = LOP ->
+      blk_in_stash id v s ->
+      kv_rel id v (write_back_r O p (length p) s).
+  Proof.
+    intros.
+    destruct (write_back_in_stash_kv_rel_aux (length p) s p id v 0 H); auto; try lia.
+    - left; auto.
+    - destruct H2 as [k [_ Hk]].
+      right.
+      eapply weaken_at_lvl_in_path.
+      rewrite calc_path_write_bk_r_stable.
+      destruct Hk.
+      eauto.
+  Qed.
+
+  Lemma distribute_via_get_post_wb_st : forall (id : block_id) (v : nat) (s : state) (p : path),
+      well_formed s ->
+      length p = LOP ->
+      blk_in_stash id v s -> 
+      kv_rel id v (get_post_wb_st s p).
+  Proof.
+    intros.
+    unfold get_post_wb_st.
+    apply write_back_in_stash_kv_rel; simpl; auto. 
+  Qed.
+
+  Lemma NoDup_path_oram : forall o p,
+      NoDup (List.map block_blockid (get_all_blks_tree o)) ->
+      NoDup (List.map block_blockid (concat (lookup_path_oram o p))).
+  Proof.
+    induction o; intros.
+    - constructor.
+    - simpl in *.
+      destruct p.
+      + destruct data.
+        * simpl.
+          rewrite app_nil_r.
+          repeat rewrite map_app in H.
+          apply NoDup_app_remove_r in H; auto.
+        * constructor.
+      + destruct b.
+        * destruct data.
+          -- simpl in *.
+             apply NoDup_disjointness.
+             ++ repeat rewrite map_app in H.
+                apply NoDup_app_remove_r in H; auto.
+             ++ apply IHo1.
+                repeat rewrite map_app in H.
+                apply NoDup_app_remove_l in H; auto.
+                apply NoDup_app_remove_r in H; auto.
+             ++ intros id [Hid1 Hid2].
+                apply In_path_in_tree in Hid2.
+                repeat rewrite map_app in H.
+                rewrite app_assoc in H.
+                apply NoDup_app_remove_r in H.
+                apply (NoDup_app_disj _ _ H id); split; auto.
+          -- apply IHo1.
+             rewrite map_app in H.
+             apply NoDup_app_remove_r in H; auto.
+        * destruct data.
+          -- simpl in *.
+             apply NoDup_disjointness.
+             ++ repeat rewrite map_app in H.
+                apply NoDup_app_remove_r in H; auto.
+             ++ apply IHo2.
+                repeat rewrite map_app in H.
+                apply NoDup_app_remove_l in H; auto.
+                apply NoDup_app_remove_l in H; auto.
+             ++ intros id [Hid1 Hid2].
+                apply In_path_in_tree in Hid2.
+                repeat rewrite map_app in H.
+                apply NoDup_app_remove_mid in H.
+                apply (NoDup_app_disj _ _ H id); split; auto.
+          -- apply IHo2.
+             rewrite map_app in H.
+             apply NoDup_app_remove_l in H; auto.
+  Qed. 
+
+  Lemma get_all_blks_tree_clear_path_weaken : forall o id p,
+      In id (List.map block_blockid (get_all_blks_tree (clear_path o p))) ->
+      In id (List.map block_blockid (get_all_blks_tree o)).
+  Proof.
+    induction o; intros.
+    - auto.
+    - destruct p; simpl in *; auto.
+      + rewrite map_app in H.
+        apply in_app_or in H.
+        destruct H.
+        * destruct data; repeat rewrite map_app.
+          -- apply in_or_app; right.
+             apply in_or_app; left; auto.
+          -- apply in_or_app; left; auto.
+        * destruct data; repeat rewrite map_app.
+          -- apply in_or_app; right.
+             apply in_or_app; right; auto.
+          -- apply in_or_app; right; auto.
+      + destruct b; simpl in *.
+        * rewrite map_app in H.
+          apply in_app_or in H.
+          destruct H.
+          -- destruct data; repeat rewrite map_app.
+             ++ apply in_or_app; right.
+                apply in_or_app; left; auto.
+                eapply IHo1; eauto.
+             ++ apply in_or_app; left.
+                eapply IHo1; eauto.
+          -- destruct data; repeat rewrite map_app.
+             ++ apply in_or_app; right.
+                apply in_or_app; right; auto.
+             ++ apply in_or_app; right; auto.
+        * destruct data; repeat rewrite map_app.
+          -- rewrite map_app in H.
+             apply in_app_or in H.
+             destruct H.
+             ++ apply in_or_app; right.
+                apply in_or_app; left; auto.
+             ++ apply in_or_app; right.
+                apply in_or_app; right.
+                eapply IHo2; eauto.
+          -- rewrite map_app in H.
+             apply in_app_or in H.
+             destruct H.
+             ++ apply in_or_app; left; auto.
+             ++ apply in_or_app; right.
+                eapply IHo2; eauto.
+  Qed.
+
+  Lemma NoDup_clear_path : forall o p,
+      NoDup (List.map block_blockid (get_all_blks_tree o)) ->
+      NoDup (List.map block_blockid (get_all_blks_tree (clear_path o p))).
+  Proof.
+    induction o; simpl in *; intros.
+    - apply NoDup_nil.
+    - destruct p; simpl.
+      + destruct data; auto.
+        repeat rewrite map_app in *.
+        apply NoDup_app_remove_l in H. auto.
+      + destruct b; simpl.
+        * apply NoDup_disjointness.
+          -- destruct data; apply IHo1.
+             ++ repeat rewrite map_app in *.
+                apply NoDup_app_remove_l in H.
+                apply NoDup_app_remove_r in H.
+                auto.
+             ++ repeat rewrite map_app in *.
+                apply NoDup_app_remove_r in H.
+                auto.
+          -- destruct data; simpl.
+             ++ repeat rewrite map_app in *.
+                apply NoDup_app_remove_l in H.
+                apply NoDup_app_remove_l in H.
+                auto.
+             ++ repeat rewrite map_app in *.
+                apply NoDup_app_remove_l in H.
+                auto.
+          -- intros id [Hid1 Hid2].
+             apply get_all_blks_tree_clear_path_weaken in Hid1.
+             destruct data; simpl.
+             ++ repeat rewrite map_app in *.
+                apply NoDup_app_remove_l in H.
+                eapply NoDup_app_disj. exact H.
+                split; eauto.
+             ++ repeat rewrite map_app in *.
+                eapply NoDup_app_disj. exact H.
+                split; eauto.
+        * apply NoDup_disjointness.
+          -- destruct data; simpl.
+             ++ repeat rewrite map_app in *.
+                apply NoDup_app_remove_l in H.
+                apply NoDup_app_remove_r in H.
+                auto.
+             ++ repeat rewrite map_app in *.
+                apply NoDup_app_remove_r in H.
+                auto.
+          -- destruct data; apply IHo2.
+             ++ repeat rewrite map_app in *.
+                apply NoDup_app_remove_l in H.
+                apply NoDup_app_remove_l in H.
+                auto.
+             ++ repeat rewrite map_app in *.
+                apply NoDup_app_remove_l in H.
+                auto.
+          -- intros id [Hid1 Hid2].
+             apply get_all_blks_tree_clear_path_weaken in Hid2.
+             destruct data; simpl.
+             ++ repeat rewrite map_app in *.
+                apply NoDup_app_remove_l in H.
+                eapply NoDup_app_disj. exact H.
+                split; eauto.
+             ++ repeat rewrite map_app in *.
+                eapply NoDup_app_disj. exact H.
+                split; eauto.
+  Qed.
+  
+  Lemma clear_path_p_b_tree : forall o n p, 
+      is_p_b_tr o n -> 
+      is_p_b_tr (clear_path o p) n.
+  Proof.
+    induction o; auto; intros.
+    destruct p.
+    - simpl.
+      destruct n.
+      + inversion H.
+      + split; destruct H; auto.
+    - destruct b; simpl.
+      destruct n.
+      + inversion H.
+      + inversion H. split.
+        * apply IHo1; auto.
+        * auto.
+      + destruct n; auto.
+        split.
+        * inversion H. auto.
+        * apply IHo2; auto. inversion H; auto.
+  Qed.
+
+  Lemma on_path_not_off_path: forall o p id,
+      NoDup (List.map block_blockid (get_all_blks_tree o)) ->
+      In id (List.map block_blockid (concat (lookup_path_oram o p))) ->
+      ~ In id (List.map block_blockid (get_all_blks_tree (clear_path o p))).
+  Proof.
+    induction o; auto; intros.
+    destruct p. 
+    - destruct data; simpl in *.
+      + repeat rewrite map_app in *.
+        apply NoDup_app_disj in H.
+        intro Hid.
+        apply (H id); split.
+        * simpl in H0.
+          rewrite app_nil_r in H0; auto.
+        * auto.
+      + auto.
+    - destruct data; simpl in *.
+      + destruct b; simpl in *.
+        * repeat rewrite map_app in *. (* true *)
+          apply in_app_or in H0.
+          destruct H0.
+          -- apply NoDup_app_disj in H.
+             intro Hid.
+             apply (H id); split; auto.
+             apply in_or_app.
+             apply in_app_or in Hid.
+             destruct Hid.
+             ++ left. eapply get_all_blks_tree_clear_path_weaken. exact H1.
+             ++ right. auto.
+          -- intro.
+             apply in_app_or in H1.
+             destruct H1. 
+             ++ apply (IHo1 p id); auto.
+                apply NoDup_app_remove_l in H.
+                apply NoDup_app_remove_r in H; auto.
+             ++ apply NoDup_app_remove_l in H.
+                apply NoDup_app_disj in H.
+                apply (H id); split; auto.
+                eapply In_path_in_tree. exact H0.
+        * repeat rewrite map_app in *. (* false *)
+          apply in_app_or in H0.
+          destruct H0.
+          -- apply NoDup_app_disj in H.
+             intro Hid.
+             apply (H id); split; auto.
+             apply in_or_app.
+             apply in_app_or in Hid.
+             destruct Hid.
+             ++ left. auto.
+             ++ right. eapply get_all_blks_tree_clear_path_weaken. exact H1.
+          -- intro.
+             apply in_app_or in H1.
+             destruct H1. 
+             ++ apply (IHo2 p id); auto.
+                ** apply NoDup_app_remove_l in H.
+                   apply NoDup_app_remove_l in H; auto.
+                ** apply NoDup_app_remove_l in H.
+                   apply NoDup_app_disj in H.
+                   elim (H id); split; auto.
+                   eapply In_path_in_tree; eauto.                 
+             ++ apply (IHo2 p id); auto.
+                apply NoDup_app_remove_l in H.
+                apply NoDup_app_remove_l in H; auto.
+      + destruct b; simpl in *.
+        * repeat rewrite map_app in *.
+          pose proof (H' := H).
+          apply NoDup_app_disj in H.
+          intro Hid.
+          apply (H id); split; auto.
+          -- eapply In_path_in_tree; eauto.
+          -- apply in_app_or in Hid.
+             destruct Hid; auto.
+             elim (IHo1 p id); auto.
+             apply NoDup_app_remove_r in H'; auto.
+        * repeat rewrite map_app in *.
+          pose proof (H' := H).
+          apply NoDup_app_disj in H.
+          intro Hid.
+          apply (H id); split; auto.
+          -- apply in_app_or in Hid.
+             destruct Hid; auto.
+             elim (IHo2 p id); auto.
+             apply NoDup_app_remove_l in H'; auto.
+          -- eapply In_path_in_tree; eauto.
+  Qed.
+
+  Lemma disjoint_list_dlt : forall o p h,
+      disjoint_list (List.map block_blockid (get_all_blks_tree o))
+        (List.map block_blockid h) ->
+      NoDup (List.map block_blockid (get_all_blks_tree o)) -> 
+      disjoint_list (List.map block_blockid (get_all_blks_tree (clear_path o p)))
+        (List.map block_blockid (concat (lookup_path_oram o p) ++ h)).
+  Proof.
+    intros.
+    intros id [Hid1 Hid2].
+    rewrite map_app in *.
+    apply in_app_or in Hid2.
+    destruct Hid2.
+    - eapply on_path_not_off_path; eauto.
+    - apply (H id); split; auto.
+      eapply get_all_blks_tree_clear_path_weaken; eauto.
+  Qed.
+  
+  Lemma disjoint_list_sub : forall {A} (l1 l2 l3: list A),
+      (forall x, In x l1 -> In x l2) -> 
+      disjoint_list l2 l3 ->
+      disjoint_list l1 l3.
+  Proof.
+    intros.
+    unfold disjoint_list in *.
+    intros. unfold not in *.
+    firstorder.
+  Qed.
+
+  Lemma lookup_update_sameid : forall id m p_new, 
+      lookup_dict
+        (makeBoolList false LOP) id
+        (update_dict id p_new m) = p_new.
+  Proof.
+    intros.
+    unfold lookup_dict.
+    unfold update_dict.
+    destruct m; simpl.
+    induction dict_elems as [|[k v] tl]; simpl.
+    - rewrite Nat.compare_refl; auto.
+    - destruct (id ?= k)%nat eqn:id_cond; simpl.
+      + rewrite Nat.compare_refl; auto.
+      + rewrite Nat.compare_refl; auto.
+      + rewrite id_cond.
+        exact IHtl.
+  Qed.
+
+  Lemma lookup_update_diffid : forall id id' m p_new,
+      id <> id' ->
+      lookup_dict
+        (makeBoolList false LOP)
+        id (update_dict id' p_new m) =
+        lookup_dict (makeBoolList false LOP) id m.
+  Proof.
+    intros.
+    unfold lookup_dict.
+    unfold update_dict.
+    destruct m; simpl.
+    induction dict_elems as [|[k v] tl]; simpl.
+    - destruct (id ?= id')%nat eqn:id_cond; auto.
+      rewrite Nat.compare_eq_iff in id_cond; contradiction.
+    - destruct (id' ?= k)%nat eqn:id_cond1; simpl.
+      + rewrite Nat.compare_eq_iff in id_cond1; subst.
+        destruct (id ?= k)%nat eqn:id_cond2; auto.
+        rewrite Nat.compare_eq_iff in id_cond2; contradiction.
+      + destruct (id ?= id')%nat eqn:id_cond2; auto.
+        * rewrite Nat.compare_eq_iff in id_cond2; contradiction.
+        * rewrite <- nat_compare_lt in *.
+          assert (id < k)%nat by lia.
+          rewrite nat_compare_lt in H0.
+          rewrite H0; auto.
+      + rewrite IHtl; auto.
+  Qed.
+
+  Lemma lookup_off_path : forall o id p p',
+      NoDup (List.map block_blockid (get_all_blks_tree o)) ->
+      In id (List.map block_blockid (get_all_blks_tree (clear_path o p))) ->
+      In id (List.map block_blockid (concat (lookup_path_oram o p'))) ->
+      In id (List.map block_blockid (concat (lookup_path_oram (clear_path o p) p'))).
+  Proof.
+    induction o; intros; simpl in *; auto.
+    destruct p; simpl in *.
+    - destruct p'.
+      + simpl.
+        destruct data; auto.
+        repeat rewrite map_app in *.
+        apply NoDup_app_disj in H.
+        simpl in H1; rewrite app_nil_r in H1.
+        apply (H id); split; auto.
+      + destruct b.
+        * destruct data; simpl in *; auto.
+          rewrite map_app in *.
+          apply in_app_or in H1.
+          destruct H1; auto.
+          apply NoDup_app_disj in H.
+          elim (H id); split; auto.
+          rewrite map_app; auto.
+        * destruct data; simpl in *; auto.
+          rewrite map_app in *.
+          apply in_app_or in H1.
+          destruct H1; auto.
+          apply NoDup_app_disj in H.
+          elim (H id); split; auto.
+          rewrite map_app; auto.
+    - destruct p'.
+      + destruct data; simpl in *.
+        * rewrite app_nil_r in H1.
+          destruct b.
+          -- simpl in *.
+             rewrite map_app in *.
+             apply NoDup_app_disj in H.
+             apply (H id); split; auto.
+             rewrite map_app.
+             rewrite in_app_iff in *.
+             destruct H0; auto.
+             left; eapply get_all_blks_tree_clear_path_weaken; eauto.
+          -- simpl in *.
+             rewrite map_app in *.
+             apply NoDup_app_disj in H.
+             apply (H id); split; auto.
+             rewrite map_app.
+             rewrite in_app_iff in *.
+             destruct H0; auto.
+             right; eapply get_all_blks_tree_clear_path_weaken; eauto.
+        * contradiction.
+      + destruct b0; simpl in *.
+        * destruct data; simpl in *.
+          -- destruct b; simpl in *.
+             ++ repeat rewrite map_app in *.
+                apply in_app_or in H1.
+                destruct H1.
+                ** apply NoDup_app_disj in H.
+                   elim (H id); split; auto.
+                   apply in_app_or in H0.
+                   apply in_or_app.
+                   destruct H0; auto.
+                   left. eapply get_all_blks_tree_clear_path_weaken; eauto.
+                ** apply IHo1; auto.
+                   --- apply NoDup_app_remove_l in H.
+                       apply NoDup_app_remove_r in H; auto.
+                   --- apply in_app_or in H0.
+                       destruct H0; auto.
+                       apply NoDup_app_remove_l in H.
+                       apply NoDup_app_disj in H.
+                       elim (H id); split; auto.
+                       eapply In_path_in_tree; eauto.
+             ++ repeat rewrite map_app in *.
+                apply in_app_or in H1.
+                destruct H1; auto.
+                apply NoDup_app_disj in H.
+                elim (H id); split; auto.
+                apply in_or_app.
+                apply in_app_or in H0.
+                destruct H0; auto.
+                right. eapply get_all_blks_tree_clear_path_weaken; eauto.
+          -- destruct b; simpl in *; auto. 
+             repeat rewrite map_app in *.
+             apply in_app_or in H0.
+             destruct H0.
+             ++ apply IHo1; auto.
+                apply NoDup_app_remove_r in H; auto.
+             ++ apply NoDup_app_disj in H.
+                elim (H id); split; auto.
+                eapply In_path_in_tree; eauto.
+        * destruct data; simpl in *.
+          -- destruct b; simpl in *.
+             ++ repeat rewrite map_app in *.
+                apply in_app_or in H1.
+                destruct H1; auto.
+                apply NoDup_app_disj in H.
+                elim (H id); split; auto.
+                apply in_or_app.
+                apply in_app_or in H0.
+                destruct H0; auto.
+                left. eapply get_all_blks_tree_clear_path_weaken; eauto.
+             ++ repeat rewrite map_app in *.
+                apply in_app_or in H1.
+                destruct H1; auto.
+                ** apply NoDup_app_disj in H.
+                   elim (H id); split; auto.
+                   apply in_or_app.
+                   apply in_app_or in H0.
+                   destruct H0; auto.
+                   right. eapply get_all_blks_tree_clear_path_weaken; eauto.
+                ** apply IHo2; auto.
+                   --- apply NoDup_app_remove_l in H.
+                       apply NoDup_app_remove_l in H; auto.
+                   --- apply in_app_or in H0.
+                       destruct H0; auto.
+                       apply NoDup_app_remove_l in H.
+                       apply NoDup_app_disj in H.
+                       elim (H id); split; auto.
+                       eapply In_path_in_tree; eauto.
+          -- destruct b; simpl in *; auto. 
+             repeat rewrite map_app in *.
+             apply in_app_or in H0.
+             destruct H0; auto.
+             ++ apply NoDup_app_disj in H.
+                elim (H id); split; auto.
+                eapply In_path_in_tree; eauto.
+             ++ apply IHo2; auto.
+                apply NoDup_app_remove_l in H; auto.
+  Qed.
+
+  Lemma rd_op_wf : forall (id : block_id) (m : position_map) (h : stash) (o : oram) (p p_new : path),
+      lookup_dict (makeBoolList false LOP) id m = p ->
+      well_formed (State m h o) -> length p_new = LOP -> 
+      well_formed
+        {|
+          state_position_map := update_dict id p_new m;
+          state_stash := (concat (lookup_path_oram o p) ++ h)%list;
+          state_oram := clear_path o p
+        |}.
+  Proof.
+    intros.
+    destruct H0.
+    constructor; simpl in *.
+    - apply NoDup_disjointness.
+      + apply NoDup_path_oram. auto.
+      + auto.
+      + apply disjoint_list_sub with
           (l2 := List.map block_blockid (get_all_blks_tree o)); auto.
-        intros. eapply In_path_in_tree. exact H.
-    + unfold blk_in_path in H. simpl in *.
-    apply in_or_app. left. auto.
-Qed.
+        intros. apply In_path_in_tree with (p := p). exact H0.
+    - apply NoDup_clear_path. auto.
+    - apply disjoint_list_dlt. auto. auto.
+    - apply clear_path_p_b_tree. auto.
+    - intros id' Hid'.
+      destruct (id =? id') eqn:id_cond.
+      + rewrite Nat.eqb_eq in id_cond. 
+        rewrite <- id_cond in *; clear id_cond.
+        pose (get_all_blks_tree_clear_path_weaken _ _ _ Hid') as Hid'2.
+        specialize (blk_in_path_in_tree0 id Hid'2).
+        rewrite H in blk_in_path_in_tree0; clear Hid'2.
+        elim on_path_not_off_path with (id := id) (o := o) (p := p); auto.
+      + rewrite Nat.eqb_neq in id_cond.
+        rewrite lookup_update_diffid; auto.
+        apply lookup_off_path; auto.
+        apply blk_in_path_in_tree0.
+        eapply get_all_blks_tree_clear_path_weaken; eauto.
+    - intro.
+      destruct (Nat.eqb id id0) eqn : id_cond.
+      + rewrite Nat.eqb_eq in id_cond. rewrite id_cond. rewrite lookup_update_sameid.
+        auto.
+      + rewrite lookup_update_diffid. auto.
+        rewrite Nat.eqb_neq in id_cond. auto.
+  Qed.
 
-Lemma read_access_wf (id : block_id)(v : nat) :
-  state_plift (fun st => @well_formed st /\ kv_rel id v st) (fun st => @well_formed st /\ kv_rel id v st) (has_value v) (read_access id).
-Proof.
-  remember (fun st : state => well_formed st /\ kv_rel id v st) as Inv. 
-  apply (state_plift_bind Inv Inv).
-  - apply state_plift_get.
-  - intros.
-    apply (state_plift_bind Inv (fun p => length p = LOP)).
-    + apply state_plift_liftT.
-      apply coin_flips_length.
-    + intros. simpl.
-      apply (state_plift_bind Inv (fun _ => True)).
-      * apply state_plift_put. rewrite HeqInv in H; destruct H.
-        rewrite HeqInv. split.
-        -- apply get_post_wb_st_wf; [|apply H].
-           apply get_pre_wb_st_wf; auto. destruct x. exact H.
-        -- apply zero_sum_stsh_tr_Rd_rev; auto. apply H. 
-      * intros. rewrite HeqInv. apply state_plift_ret.
-        rewrite HeqInv in H. destruct H. simpl.
-        symmetry. apply zero_sum_stsh_tr_Rd; destruct x; auto.
-Qed.
+  Lemma not_in_removed : forall l id,
+      ~ In id
+        (List.map block_blockid
+           (remove_list (fun blk : block => block_blockid blk =? id)
+              l)).
+  Proof.
+    intros.
+    rewrite in_map_iff.
+    intros [b [Hb1 Hb2]].
+    rewrite In_remove_list_iff in Hb2.
+    destruct Hb2 as [_ Hb2].
+    rewrite Hb1 in Hb2.
+    simpl in Hb2.
+    rewrite Nat.eqb_neq in Hb2.
+    contradiction.
+  Qed.
 
-Lemma write_access_wf (id : block_id) (v : nat) :
-  state_plift (fun st => @well_formed st) (fun st => @well_formed st /\ kv_rel id v st) (fun _ => True) (write_access id v).
-Proof.
-  remember (fun st : state => well_formed st) as Inv.
-  apply (state_plift_bind Inv Inv).
-  - apply state_plift_get.
-  - intros.
-    rewrite HeqInv in H.
-    apply (state_plift_bind Inv (fun p => length p = LOP)).
-    + apply state_plift_liftT.
-      apply coin_flips_length.
-    + intros. simpl.
-      apply (state_plift_bind (fun st => @well_formed st /\ kv_rel id v st) (fun _ => True)).
-      * apply state_plift_put; simpl; split.
-        apply get_post_wb_st_wf; auto.
-        -- apply get_pre_wb_st_wf; auto. destruct x; exact H.
-        -- apply H.
-        -- apply zero_sum_stsh_tr_Wr; auto. 
-           apply H.
-      * intros. rewrite HeqInv. eapply state_plift_ret. auto.
-Qed.
+  Lemma NoDup_remove_list: forall l id,
+      NoDup (List.map block_blockid l) -> 
+      NoDup
+        (List.map block_blockid
+           (remove_list (fun blk : block => block_blockid blk =? id)
+              l)).
+  Proof.
+    induction l; simpl; intros; auto.
+    destruct (block_blockid a =? id).
+    - apply IHl; auto.
+      inversion H; auto.
+    - simpl.
+      constructor.
+      + intro pf.
+        rewrite in_map_iff in pf.
+        destruct pf as [b [Hb1 Hb2]].
+        rewrite In_remove_list_iff in Hb2.
+        destruct Hb2 as [Hb2 Hb3].
+        inversion H.
+        rewrite <- Hb1 in H2.
+        apply H2.
+        apply in_map; auto.
+      + apply IHl.
+        inversion H; auto.
+  Qed.
+  
+  Lemma wr_op_wf : forall (id : block_id) (v : nat) (m : position_map) (h : stash) (o : oram) (p p_new : path),
+      well_formed (State m h o) -> length p_new = LOP ->
+      lookup_dict (makeBoolList false LOP) id m = p ->
+      well_formed
+        {|
+          state_position_map := update_dict id p_new m;
+          state_stash :=
+            {| block_blockid := id; block_payload := v |}
+              :: remove_list (fun blk : block => block_blockid blk =? id)
+              (concat (lookup_path_oram o p) ++ h);
+          state_oram := clear_path o p
+        |}.
+  Proof.
+    intros.
+    destruct H.
+    constructor; simpl in *.
+    - rewrite NoDup_cons_iff; split.
+      + apply not_in_removed.
+      + apply NoDup_remove_list.
+        apply NoDup_disjointness; auto.
+        * apply NoDup_path_oram; auto.
+        * eapply disjoint_list_sub.
+          -- apply In_path_in_tree.
+          -- auto.
+    - apply NoDup_clear_path. auto.
+    - intros id' [Hid'1 Hid'2].
+      destruct Hid'2.
+      + rewrite <- H in Hid'1; clear H.
+        apply on_path_not_off_path with (id := id) (o := o) (p := p); auto.
+        rewrite <- H1.
+        apply blk_in_path_in_tree0.
+        eapply get_all_blks_tree_clear_path_weaken; eauto.
+      + eapply disjoint_list_dlt; eauto; split; eauto.
+        rewrite in_map_iff in *.
+        destruct H as [b [Hb1 Hb2]].
+        exists b; split; auto.
+        rewrite In_remove_list_iff in Hb2; destruct Hb2; auto.
+    - apply clear_path_p_b_tree. auto.
+    - intros id' Hid'.
+      destruct (id =? id') eqn:id_cond.
+      + rewrite Nat.eqb_eq in id_cond. 
+        rewrite <- id_cond in *; clear id_cond.
+        pose (get_all_blks_tree_clear_path_weaken _ _ _ Hid') as Hid'2.
+        specialize (blk_in_path_in_tree0 id Hid'2).
+        rewrite H1 in blk_in_path_in_tree0; clear Hid'2.
+        elim on_path_not_off_path with (id := id) (o := o) (p := p); auto.
+      + rewrite Nat.eqb_neq in id_cond.
+        rewrite lookup_update_diffid; auto.
+        apply lookup_off_path; auto.
+        apply blk_in_path_in_tree0.
+        eapply get_all_blks_tree_clear_path_weaken; eauto.
+    - intro.
+      destruct (Nat.eqb id id0) eqn : id_cond.
+      + rewrite Nat.eqb_eq in id_cond. rewrite id_cond. rewrite lookup_update_sameid.
+        auto.
+      + rewrite lookup_update_diffid. auto.
+        rewrite Nat.eqb_neq in id_cond. auto.
+  Qed.
 
-(*
- * this lemma is saying that the write_and_read_access preserves the well-formedness invariant
- * and returns the correct value
- *)
+  Lemma get_pre_wb_st_wf : forall (id : block_id) (op : operation) (m : position_map) (h : stash) (o : oram) (p p_new : path),
+      well_formed (State m h o) ->
+      length p_new = LOP ->
+      lookup_dict (makeBoolList false LOP) id m = p ->    
+      well_formed (get_pre_wb_st id op m h o p p_new).
+  Proof.
+    intros.
+    unfold get_pre_wb_st.
+    destruct op. 
+    - simpl. apply rd_op_wf; auto.
+    - simpl. apply wr_op_wf; auto.
+  Qed.
 
-Lemma write_and_read_access_lift (id : block_id)(v : nat):
-  state_plift (@well_formed) well_formed (has_value v)
-                  (write_and_read_access id v).
-Proof.
-  apply (state_plift_bind
-           (fun st => well_formed st /\ kv_rel id v st)
-           (fun _ => True)).
-  - eapply write_access_wf.
-  - intros _ _.
-    apply (state_plift_weaken (fun st : state => well_formed st /\ kv_rel id v st)).
-    + exact dist_has_weakening.
-    + tauto.
-    + apply read_access_wf.
-Qed.
+  Lemma get_post_wb_st_wf : forall (s : state) (p : path),
+      well_formed s ->
+      length p = LOP ->
+      well_formed (get_post_wb_st s p).
+  Proof.
+    intros.
+    unfold get_post_wb_st.
+    apply write_back_wf; auto; lia.
+  Qed.
 
-Lemma extract_payload (id : block_id) (v: nat) (s : state) : 
-  plift (fun '(x, s') => has_value v x /\ well_formed s') (write_and_read_access id v s) -> 
-  get_payload (write_and_read_access id v s) = v.
-Proof.
-  intros ops_on_s.
-  unfold get_payload.
-  apply dist_lift_peek in ops_on_s.
-  destruct peek.
-  destruct p.
-  destruct ops_on_s; congruence.
-Qed.
+  Lemma zero_sum_stsh_tr_Wr
+    (s : state) (id : block_id) (v : nat) (p p_new : path):
+    well_formed s ->
+    length p = LOP ->
+    length p_new = LOP ->
+    kv_rel id v
+      (get_post_wb_st
+         (get_pre_wb_st id (Write v)
+            (state_position_map s) (state_stash s) (state_oram s)
+            (calc_path id s) p_new) p).
+  Proof.
+    intros.
+    apply distribute_via_get_post_wb_st; auto.
+    - apply get_pre_wb_st_wf; auto.
+      destruct s; auto.
+    - apply stash_path_combined_rel_Wr.
+  Qed.
+  
+  Lemma zero_sum_stsh_tr_Rd_rev :
+    forall (id : block_id) (v : nat) (s : state) (p p_new : path),
+      well_formed s ->
+      length p = LOP ->
+      length p_new = LOP -> 
+      kv_rel id v s  -> 
+      kv_rel id v (get_post_wb_st
+                     (get_pre_wb_st id Read (state_position_map s)
+                        (state_stash s)
+                        (state_oram s)
+                        (calc_path id s) p_new) p). 
+  Proof.
+    intros.
+    apply distribute_via_get_post_wb_st; auto.
+    - apply get_pre_wb_st_wf; auto. destruct s; auto.
+    - apply stash_path_combined_rel_Rd. auto.
+  Qed.
+  
+  Lemma lookup_ret_data_block_in_list (id : block_id) (v : nat) (l : list block) :
+    NoDup (List.map block_blockid l) ->
+    In (Block id v) l -> lookup_ret_data id l = v.
+  Proof.
+    intro ND.
+    intros.
+    induction l; simpl; try contradiction.
+    destruct (block_blockid a =? id) eqn: id_cond.
+    - destruct H; simpl in *.
+      + rewrite H; auto.
+      + inversion ND; subst.
+        rewrite Nat.eqb_eq in id_cond.
+        rewrite id_cond in H2.
+        apply List.in_map with (f := block_blockid) in H.
+        simpl in *. contradiction.
+    - apply IHl.
+      + inversion ND; auto.
+      + destruct H; auto.
+        rewrite H in id_cond. simpl in *. rewrite Nat.eqb_neq in id_cond.
+        contradiction.
+  Qed.
 
-Theorem PathORAM_simulates_RAM (id : block_id) (v : nat) (s : state) :
-  well_formed s ->
+  Lemma zero_sum_stsh_tr_Rd (id : block_id) (v : nat) (m : position_map) (h : stash) (o : oram) :
+    well_formed (State m h o) ->
+    kv_rel id v (State m h o) ->
+    get_ret_data id h (calc_path id (State m h o)) o = v.
+  Proof.
+    simpl.
+    intros.
+    destruct H0. 
+    - (* assume in stash *)
+      apply lookup_ret_data_block_in_list.
+      + apply NoDup_disjointness; try repeat apply H.
+        * apply NoDup_path_oram. apply H.
+        * destruct H.
+          apply disjoint_list_sub with
+            (l2 := List.map block_blockid (get_all_blks_tree o)); auto.
+          intros. eapply In_path_in_tree. exact H.
+      + apply in_or_app. right. auto.
+    - (* assume in path *)
+      apply lookup_ret_data_block_in_list.
+      + apply NoDup_disjointness; try repeat apply H.
+        * apply NoDup_path_oram. apply H.
+        * destruct H.
+          apply disjoint_list_sub with
+            (l2 := List.map block_blockid (get_all_blks_tree o)); auto.
+          intros. eapply In_path_in_tree. exact H.
+      + unfold blk_in_path in H. simpl in *.
+        apply in_or_app. left. auto.
+  Qed.
+
+  Lemma read_access_wf (id : block_id)(v : nat) :
+    state_plift (fun st => @well_formed st /\ kv_rel id v st) (fun st => @well_formed st /\ kv_rel id v st) (has_value v) (read_access id).
+  Proof.
+    remember (fun st : state => well_formed st /\ kv_rel id v st) as Inv. 
+    apply (state_plift_bind Inv Inv).
+    - apply state_plift_get.
+    - intros.
+      apply (state_plift_bind Inv (fun p => length p = LOP)).
+      + apply state_plift_liftT.
+        apply coin_flips_length.
+      + intros. simpl.
+        apply (state_plift_bind Inv (fun _ => True)).
+        * apply state_plift_put. rewrite HeqInv in H; destruct H.
+          rewrite HeqInv. split.
+          -- apply get_post_wb_st_wf; [|apply H].
+             apply get_pre_wb_st_wf; auto. destruct x. exact H.
+          -- apply zero_sum_stsh_tr_Rd_rev; auto. apply H. 
+        * intros. rewrite HeqInv. apply state_plift_ret.
+          rewrite HeqInv in H. destruct H. simpl.
+          symmetry. apply zero_sum_stsh_tr_Rd; destruct x; auto.
+  Qed.
+
+  Lemma write_access_wf (id : block_id) (v : nat) :
+    state_plift (fun st => @well_formed st) (fun st => @well_formed st /\ kv_rel id v st) (fun _ => True) (write_access id v).
+  Proof.
+    remember (fun st : state => well_formed st) as Inv.
+    apply (state_plift_bind Inv Inv).
+    - apply state_plift_get.
+    - intros.
+      rewrite HeqInv in H.
+      apply (state_plift_bind Inv (fun p => length p = LOP)).
+      + apply state_plift_liftT.
+        apply coin_flips_length.
+      + intros. simpl.
+        apply (state_plift_bind (fun st => @well_formed st /\ kv_rel id v st) (fun _ => True)).
+        * apply state_plift_put; simpl; split.
+          apply get_post_wb_st_wf; auto.
+          -- apply get_pre_wb_st_wf; auto. destruct x; exact H.
+          -- apply H.
+          -- apply zero_sum_stsh_tr_Wr; auto. 
+             apply H.
+        * intros. rewrite HeqInv. eapply state_plift_ret. auto.
+  Qed.
+
+  (*
+   * this lemma is saying that the write_and_read_access preserves the well-formedness invariant
+   * and returns the correct value
+   *)
+
+  Lemma write_and_read_access_lift (id : block_id)(v : nat):
+    state_plift (@well_formed) well_formed (has_value v)
+      (write_and_read_access id v).
+  Proof.
+    apply (state_plift_bind
+             (fun st => well_formed st /\ kv_rel id v st)
+             (fun _ => True)).
+    - eapply write_access_wf.
+    - intros _ _.
+      apply (state_plift_weaken (fun st : state => well_formed st /\ kv_rel id v st)).
+      + exact dist_has_weakening.
+      + tauto.
+      + apply read_access_wf.
+  Qed.
+
+  Lemma extract_payload (id : block_id) (v: nat) (s : state) : 
+    plift (fun '(x, s') => has_value v x /\ well_formed s') (write_and_read_access id v s) -> 
+    get_payload (write_and_read_access id v s) = v.
+  Proof.
+    intros ops_on_s.
+    unfold get_payload.
+    apply dist_lift_peek in ops_on_s.
+    destruct peek.
+    destruct p.
+    destruct ops_on_s; congruence.
+  Qed.
+
+  Theorem PathORAM_simulates_RAM (id : block_id) (v : nat) (s : state) :
+    well_formed s ->
     get_payload(write_and_read_access id v s) = v.
-Proof.
-  intros wf_s.
-  apply extract_payload.
-  apply write_and_read_access_lift. auto.
-Qed.
+  Proof.
+    intros wf_s.
+    apply extract_payload.
+    apply write_and_read_access_lift. auto.
+  Qed.
 
 End PORAM_PROOF.
